current-formalism/Util/MMultiset/MMultisetWMap.v
@@ -9,110 +9,210 @@
 (******************************************)
 
 
-Require Import MMapInterface.
+(* Require Import MMapInterface. *)
 Require Import Arith_base.
 Require Import Omega.
 Require Import PArith.
+Require Import Bool.
 Require Import RelationPairs.
+Require Import SetoidList.
+Require Import Pactole.Util.FMaps.FMapInterface.
+Require Import Pactole.Util.FMaps.FMapFacts.
 Require Import Pactole.Util.MMultiset.Preliminary.
 Require Import Pactole.Util.MMultiset.MMultisetInterface.
-Require Export Pactole.Util.FMaps.FMapInterface.
 Require Import SetoidDec.
 
 
+Section WMapImplementation.
+Context (elt : Type).
+Context (elt_Setoid : Setoid elt).
+Context (elt_EqDec : @EqDec elt elt_Setoid).
+Context (MapImpl : @FMap elt elt_Setoid elt_EqDec).
+Context (MapSpec : FMapSpecs MapImpl).
 
-Definition multiplicity elt {elt_Setoid : Setoid elt} {elt_EqDec : @EqDec elt elt_Setoid}
-                            {Mapimpl : @FMap elt elt_Setoid elt_EqDec} :=
+Definition multiplicity :=
   fun x m => match find x m with Some n => Pos.to_nat n | None => 0 end.
-Check multiplicity.
+Definition m_add := fun x n m =>
+    if eq_nat_dec n 0 then m else FMapInterface.add x (Pos.of_nat (multiplicity x m + n)) m.
+Definition m_fold := fun {A} (f : elt -> nat -> A -> A) m =>
+  FMapInterface.fold (fun x y => f x (Pos.to_nat y)) m.
 
-Instance FMultisets elt (elt_Setoid : Setoid elt) `(elt_EqDec : @EqDec elt elt_Setoid)
-                        (Mapimpl : @FMap elt elt_Setoid elt_EqDec) : FMOps elt elt_EqDec := {|
+Instance pre_multiplicity_compat : Proper (equiv ==> Equal ==> Logic.eq) multiplicity.
+Proof.
+intros x y Hxy m m' Hm. unfold multiplicity. rewrite Hm.
+assert (Heq : find x m' = find y m') by now apply find_m.
+now rewrite Heq.
+Qed.
+
+Instance m_add_compat : Proper (equiv ==> Logic.eq ==> Equal ==> Equal) m_add.
+Proof.
+intros x y Hxy ? n ? m m' Hm z. subst. unfold m_add.
+destruct (Nat.eq_dec n 0).
+- apply Hm.
+- cbn. apply add_m; trivial. do 2 f_equal. rewrite Hxy. unfold multiplicity. now rewrite Hm.
+Qed.
+
+Lemma m_add_same : forall x n s, multiplicity x (m_add x n s) = n + multiplicity x s.
+Proof.
+intros x n s. unfold m_add. destruct (Nat.eq_dec n 0). omega.
+unfold multiplicity at 1. rewrite add_eq_o, Nat2Pos.id; omega || reflexivity.
+Qed.
+
+Lemma m_add_other : forall x y n s, x =/= y -> multiplicity x (m_add y n s) = multiplicity x s.
+Proof.
+intros x y n s Hyx. unfold add. simpl. unfold m_add. destruct (Nat.eq_dec n 0); trivial; [].
+unfold multiplicity at 1 3. rewrite add_neq_o; reflexivity || now symmetry.
+Qed.
+
+Lemma fold_add_out_list : forall (f : elt -> positive -> positive) x n l s,
+  ~InA eq_key (x, n) l -> NoDupA eq_key l ->
+  multiplicity x (fold_left (fun acc xn => m_add (fst xn) (Pos.to_nat (f (fst xn) (snd xn))) acc) l s)
+  = multiplicity x s.
+Proof.
+intros f x n l s Hin Hdup. revert s. induction l as [| [y m] l]; intro s; simpl.
++ reflexivity.
++ rewrite IHl.
+  - rewrite m_add_other; trivial. intro. apply Hin. now left.
+  - auto.
+  - now inversion_clear Hdup.
+Qed.
+
+Lemma fold_add_out : forall (f : elt -> nat -> nat) x s s', ~FMapInterface.In x s ->
+  multiplicity x (m_fold (fun y n acc => m_add y (f y n) acc) s s') = multiplicity x s'.
+Proof.
+intros f x s s' Hin. unfold m_fold. rewrite FMapInterface.fold_1.
+assert (Hs : forall n, ~(InA eq_key_elt (x, n) (FMapInterface.elements s))).
+{ intros n Habs. apply Hin. exists n. now apply elements_2. }
+revert s'. induction (FMapInterface.elements s) as [| [y m] l]; intro s'; simpl.
++ reflexivity.
++ assert ( Hxy : x =/= y). { intro Habs. apply (Hs m). left. now split. }
+  rewrite IHl.
+  - now rewrite m_add_other.
+  - intros n Habs. apply (Hs n). now right.
+Qed.
+
+Notation compatb := (Proper (@equiv elt _ ==> Logic.eq ==> Logic.eq)) (only parsing).
+
+Lemma fold_add : forall (f : elt -> nat -> nat) x n m m', compatb f -> find x m = Some n ->
+  multiplicity x (m_fold (fun x n acc => m_add x (f x n) acc) m m')
+  = f x (Pos.to_nat n) + multiplicity x m'.
+Proof.
+intros f x n m m' Hf Hin. unfold m_fold. rewrite fold_1.
+assert (Hm : InA eq_key_elt (x, Pos.of_nat (multiplicity x m)) (FMapInterface.elements m)).
+{ apply elements_1. rewrite find_mapsto_iff. unfold multiplicity in *.
+  destruct (find x m); discriminate || now rewrite Pos2Nat.id. }
+assert (Hdup := elements_3 m).
+revert m'. induction (FMapInterface.elements m) as [| [y p] l]; intro m'; simpl; [now inversion Hm |].
+destruct (equiv_dec x y) as [Hxy | Hxy].
+* assert (p = Pos.of_nat (multiplicity x m)).
+  { inversion_clear Hm. destruct H as [H1 H2]; try now cbn in H1, H2.
+    eapply InA_impl_compat in H; try apply eq_key_elt_eq_key_subrelation || reflexivity.
+    inversion_clear Hdup. elim H0. rewrite <- Hxy. revert H. apply InA_compat; autoclass. reflexivity. }
+  subst p.
+(*  assert (Hn : multiplicity x m = Pos.to_nat n). { unfold multiplicity. now rewrite Hin. }
+  transitivity (multiplicity x (fold_left (fun acc xn =>
+    m_add (fst xn) (Pos.to_nat (Pos.of_nat (f (fst xn) (Pos.to_nat (snd xn))))) acc) l m')).
+  + destruct (f x (Pos.to_nat n)) eqn:Hfxn.
+    - assert (Heq : Equal (m_add y (f y (Pos.to_nat (Pos.of_nat (multiplicity x m)))) m') m').
+      { intro. unfold m_add. rewrite Hxy in Hfxn. rewrite Hn, Pos2Nat.id.
+        destruct (Nat.eq_dec (f y (Pos.to_nat n)) 0) as [Heq | Heq]; trivial. rewrite Hfxn in *. now elim Heq. }
+      f_equiv. apply (fold_left_extensional (eqA:=eq_key_elt) (eqB:=Equal)); [| reflexivity | assumption].
+      intros ? ? Heq1 xn yp Heq2. unfold m_add.
+      destruct (Nat.eq_dec (f (fst xn) (Pos.to_nat (snd xn))) 0) eqn:Hfyn.
+      
+ f_equiv; trivial; try (now destruct Heq2); [].
+      
+ rewrite Nat2Pos.id.
+      -- rewrite Heq1. destruct Heq2 as [Heq2 Heq3]. cbn in Heq2, Heq3. now rewrite Heq2, Heq3.
+      -- 
+  + transitivity (multiplicity x (fold_left (fun acc xn =>
+      m_add (fst xn) (Pos.to_nat (Pos.of_nat (f (fst xn) (Pos.to_nat (snd xn))))) acc) l
+     (m_add y (f y (Pos.to_nat (Pos.of_nat (multiplicity x m)))) m'))).
+    - f_equiv. apply (fold_left_extensional (eqA:=eq_key_elt) (eqB:=Equal)); [| reflexivity | reflexivity].
+      intros ? ? Heq ? ? Heq'. rewrite Nat2Pos.id.
+      -- rewrite Heq. destruct Heq' as [Heq1 Heq2]. cbn in Heq1, Heq2. now rewrite Heq1, Heq2.
+      -- 
+  + rewrite (fold_add_out_list (fun x n => Pos.of_nat (f x (Pos.to_nat n))) x n l _).
+    - assert (multiplicity x m = Pos.to_nat n). { unfold multiplicity. now rewrite Hin. }
+      rewrite Hxy, m_add_same. do 2 f_equal. rewrite <- Hxy, H, Nat2Pos.id; trivial.
+      intro Habs. elim (lt_irrefl 0). rewrite <- Habs at 2. apply Pos2Nat.is_pos.
+    - inversion_clear Hdup. intro Habs. apply H. revert Habs. apply InA_eqA; autoclass.
+    - now inversion_clear Hdup.
+* rewrite IHl.
+  + f_equal. now apply m_add_other.
+  + inversion_clear Hm; trivial. now destruct H as [? _].
+  + now inversion_clear Hdup.
+Qed. *)
+Admitted.
+
+
+Instance FMOps_WMap : FMOps elt elt_EqDec := {|
   multiset := Map[elt, positive];
   MMultisetInterface.empty := FMapInterface.empty positive;
   MMultisetInterface.is_empty := FMapInterface.is_empty;
-  MMultisetInterface.multiplicity := multiplicity elt;
-  MMultisetInterface.add := fun x n m => if eq_nat_dec n 0 then m else add x (Pos.of_nat (m[x] + n)) m;
-  MMultisetInterface.singleton x n := add x n empty |}.
+  MMultisetInterface.multiplicity := multiplicity;
+  MMultisetInterface.add := m_add;
+  MMultisetInterface.singleton x n :=
+    if eq_nat_dec n 0 then FMapInterface.empty _ else FMapInterface.add x (Pos.of_nat n) (FMapInterface.empty _);
   remove x n m := if eq_nat_dec n 0 then m else
-    if le_lt_dec m[x] n then remove x m else add x (Pos.of_nat (multiplicity x s - n)) s.
-Definition union (s s' : t) := M.fold (fun x n acc => add x (Pos.to_nat n) acc) s s'.
-Definition inter (s s' : t) :=
-  M.fold (fun x n acc => add x ((fun x n => min (multiplicity x s) (Pos.to_nat n)) x n) acc) s' empty.
-Definition diff (s s' : t) := M.fold (fun x n acc => add x (Pos.to_nat n - multiplicity x s') acc) s empty.
-Definition lub (s s' : t) := M.fold (fun x n acc => add x (Pos.to_nat n - multiplicity x s') acc) s s'.
-Definition equal (s s' : t) := M.equal Pos.eqb s s'.
-Definition subset s s' := is_empty (diff s s').
-Definition fold {A} f (s : t) := @M.fold positive A (fun x y => f x (Pos.to_nat y)) s.
-Definition for_all f (s : t) := M.fold (fun x n b => b && f x (Pos.to_nat n)) s true.
-Definition exists_ f (s : t) := M.fold (fun x n b => b || f x (Pos.to_nat n)) s false.
-Definition nfilter f (s : t) :=
-  M.fold (fun x n acc => if f x (Pos.to_nat n) : bool then add x (Pos.to_nat n) acc else acc) s empty.
-Definition filter f (s : t) := nfilter (fun x _ => f x) s.
-Definition npartition f (s : t) :=
-  M.fold (fun x n acc => if f x (Pos.to_nat n) : bool then (add x (Pos.to_nat n) (fst acc), snd acc)
-                                               else (fst acc, add x (Pos.to_nat n) (snd acc))) s (empty,empty).
-Definition partition f (s : t) := npartition (fun x _ => f x) s.
-Definition cardinal (s : t) := M.fold (fun _ n acc => Pos.to_nat n + acc) s 0.
-Definition size (s : t) := M.fold (fun _ _ n => S n) s 0.
-Definition elements (s : t) := List.map (fun xy => (fst xy, Pos.to_nat (snd xy))) (M.bindings s).
-Definition support (s : t) := M.fold (fun x _ l => cons x l) s nil.
-Definition choose (s : t) := M.fold (fun x _ _ => Some x) s None.
-    add : elt -> nat -> multiset -> multiset;
-    singleton : elt -> nat -> multiset;
-    remove : elt -> nat -> multiset -> multiset;
-    union : multiset -> multiset -> multiset;
-    inter : multiset -> multiset -> multiset;
-    diff : multiset -> multiset -> multiset;
-    lub : multiset -> multiset -> multiset;
-    equal : multiset -> multiset -> bool;
-    subset : multiset -> multiset -> bool;
-    fold : forall A : Type, (elt -> nat -> A -> A) -> multiset -> A -> A;
-    for_all : (elt -> nat -> bool) -> multiset -> bool;
-    exists_ : (elt -> nat -> bool) -> multiset -> bool;
-    nfilter : (elt -> nat -> bool) -> multiset -> multiset;
-    filter : (elt -> bool) -> multiset -> multiset;
-    npartition : (elt -> nat -> bool) -> multiset -> multiset * multiset;
-    partition : (elt -> bool) -> multiset -> multiset * multiset;
-    elements : multiset -> list (elt * nat);
-    support : multiset -> list elt;
-    cardinal : multiset -> nat;
-    size : multiset -> nat;
-    choose : multiset -> option elt }
-
-
-Definition eq_pair := RelProd E.eq (@Logic.eq nat).
-Definition eq_elt := RelCompFun E.eq (@fst E.t nat).
-
-
-Instance Meq_equiv A : Equivalence (@M.eq_key_elt A).
-Proof. split.
-  intro. reflexivity.
-  intros ? ?. now symmetry.
-  intros ? y ? ? ?. now transitivity y.
-Qed.
-
-Instance Meq_key_equiv A : Equivalence (@M.eq_key A).
-Proof. split.
-  intro. reflexivity.
-  intros ? ?. now symmetry.
-  intros ? y ? ? ?. now transitivity y.
-Qed.
+    if le_lt_dec (multiplicity x m) n then FMapInterface.remove x m
+    else FMapInterface.add x (Pos.of_nat (multiplicity x m - n)) m;
+  union := fun m m' => m_fold m_add m m';
+  inter := fun m m' => m_fold (fun x n acc => m_add x (min (multiplicity x m) n) acc) m' (FMapInterface.empty _);
+  diff := fun m m' => m_fold (fun x n acc => m_add x (n - multiplicity x m') acc) m (FMapInterface.empty _);
+  lub := fun m m' => m_fold (fun x n acc => m_add x (n - (multiplicity x m')) acc) m m';
+  equal := fun m m' => FMapInterface.equal Pos.eqb m m';
+  subset := fun m m' => FMapInterface.is_empty
+              (m_fold (fun x n acc => m_add x (n - multiplicity x m') acc) m (FMapInterface.empty _));
+  fold := @m_fold;
+  for_all := fun f m => m_fold (fun x n b => b && f x n) m true;
+  exists_ := fun f m => m_fold (fun x n b => b || f x n) m false;
+  nfilter := fun f m => m_fold (fun x n acc => if f x n then m_add x n acc else acc) m (FMapInterface.empty _);
+  filter := fun f m => m_fold (fun x n acc => if f x then m_add x n acc else acc) m (FMapInterface.empty _);
+  npartition := fun (f : elt -> nat -> bool) m => m_fold
+                  (fun x n acc => if f x n then (m_add x n (fst acc), snd acc) else (fst acc, m_add x n (snd acc)))
+                  m (FMapInterface.empty _, FMapInterface.empty _);
+  partition := fun (f : elt -> bool) m => m_fold
+                 (fun x n acc => if f x then (m_add x n (fst acc), snd acc) else (fst acc, m_add x n (snd acc)))
+                  m (FMapInterface.empty _, FMapInterface.empty _);
+  elements := fun m => List.map (fun xy => (fst xy, Pos.to_nat (snd xy))) (FMapInterface.elements m);
+  support := fun m => FMapInterface.fold (fun x _ l => cons x l) m nil;
+  cardinal := fun m => FMapInterface.fold (fun _ n acc => Pos.to_nat n + acc) m 0;
+  size := fun m => FMapInterface.fold (fun _ _ n => S n) m 0;
+  choose := fun m =>  FMapInterface.fold (fun x _ _ => Some x) m None |}.
 
 Instance eq_pair_equiv : Equivalence eq_pair.
 Proof. split. easy. easy. intros ? y ? ? ?. now transitivity y. Qed.
 
-Lemma Meq_dec : forall x y : E.t * positive, {M.eq_key_elt x y} + {~M.eq_key_elt x y}.
+Instance eq_pair_Setoid : Setoid (elt * positive)%type := _.
+
+Instance eq_pair_EqDec : @EqDec (elt * positive)%type _.
 Proof.
-intros [t1 n1] [t2 n2].
-destruct (E.eq_dec t1 t2). destruct (Pos.eq_dec n1 n2).
-  left. now split.
-  right. intros []. contradiction.
-  right. intros []. contradiction.
+intros [x n] [y p]. destruct (equiv_dec x y).
++ destruct (Pos.eq_dec n p).
+  - left. now split; cbn.
+  - right. intro Heq. now destruct Heq.
++ right. intro Heq. now destruct Heq.
 Defined.
 
-Lemma eq_key_elt_eq_key_weak_In B : forall x y n m l, 
-  E.eq x y -> InA (@M.eq_key_elt B) (x, n) l -> InA (@M.eq_key B) (y, m) l.
+Instance eq_elt_equiv : Equivalence eq_elt.
+Proof. split. easy. easy. intros ? y ? ? ?. now transitivity y. Qed.
+
+Instance eq_elt_Setoid : Setoid (elt * nat)%type := {| equiv := eq_elt; setoid_equiv := _ |}.
+
+Instance eq_elt_EqDec : @EqDec (elt * nat)%type _.
+Proof.
+intros [x n] [y p]. destruct (equiv_dec x y); now left + right; cbn.
+Defined.
+
+Instance eq_pair_elt_subrelation : subrelation eq_pair eq_elt.
+Proof. intros x y [H _]. apply H. Qed.
+
+Instance eq_key_eq_key_elt_subrelation : subrelation (@eq_key_elt elt _ _ _ positive) eq_key.
+Proof. intros x y [H _]. apply H. Qed.
+
+Lemma eq_pair_elt_weak_In : forall x y n m l,
+  x == y -> InA eq_pair (x, n) l -> InA eq_elt (y, m) l.
 Proof.
 intros x y n m l Heq Hin. induction l.
 + now inversion Hin.
@@ -121,391 +221,256 @@ intros x y n m l Heq Hin. induction l.
   - right. now apply IHl.
 Qed.
 
-Lemma NoDup_pair_In : forall A x y n m l, NoDupA (@M.eq_key A) l ->
-  InA (@M.eq_key_elt _) (x, n) l -> InA (@M.eq_key_elt _) (y, m) l -> E.eq x y -> n = m.
+Lemma NoDup_pair_In : forall x y n m l, NoDupA eq_elt l ->
+  InA eq_pair (x, n) l -> InA eq_pair (y, m) l -> x == y -> n = m.
 Proof.
-intros A x y n m l Hl Hinx Hiny Heq. induction Hl as [| [z p] l]. inversion_clear Hiny.
+intros x y n m l Hl Hinx Hiny Heq. induction Hl as [| [z p] l]. inversion_clear Hiny.
 inversion_clear Hinx; inversion_clear Hiny.
 - compute in H0, H1. destruct H0 as [H0 ?], H1 as [H1 ?]. now subst p m.
 - compute in H0. destruct H0 as [H0 ?]. subst p. elim H.
-  apply eq_key_elt_eq_key_weak_In with y m. now transitivity x. assumption.
+  apply eq_pair_elt_weak_In with y m. now transitivity x. assumption.
 - compute in H1. destruct H1 as [H1 ?]. subst p. elim H.
-  apply eq_key_elt_eq_key_weak_In with x n. now transitivity y; auto. assumption.
+  apply eq_pair_elt_weak_In with x n. now transitivity y; auto. assumption.
 - now apply IHHl.
 Qed.
 
-Lemma Melements_InA : forall A x n s, InA (@M.eq_key_elt A) (x, n) (M.bindings s) <-> M.MapsTo x n s.
-Proof. intros. now apply M.bindings_spec1. Qed.
+Notation "s  [c=]  t" := (Subset s t) (at level 70, no associativity).
 
-Instance Mfind_compat {A} : Proper (E.eq ==> @M.Equal A ==> Logic.eq) (@M.find A).
+Instance multiset_Setoid : Setoid multiset := {| equiv := fun m m' => forall x, m[x] = m'[x] |}.
+Proof. split; repeat intro; solve [ eauto | etransitivity; eauto ]. Defined.
+
+Instance multiplicity_compat : Proper (equiv ==> equiv ==> Logic.eq) MMultisetInterface.multiplicity.
 Proof.
-intros x1 x2 Hx s1 s2 Hs. rewrite Hs. clear s1 Hs. destruct (M.find x1 s2) eqn:Hin.
-- rewrite M.find_spec, Hx, <- M.find_spec in Hin. auto.
-- destruct (M.find x2 s2) eqn:Hin'; trivial. rewrite M.find_spec, <- Hx, <- M.find_spec, Hin in Hin'. discriminate.
+intros x y Hxy m m' Hm. rewrite Hm. simpl. unfold multiplicity.
+assert (Heq : find x m' = find y m') by now apply find_m.
+now rewrite Heq.
 Qed.
 
-Definition elt := E.t.
-Definition t := M.t positive.
-
-Definition empty : t := @M.empty positive.
-Definition is_empty (s : t) := M.is_empty s.
-Definition multiplicity x (s : t) := match M.find x s with Some n => Pos.to_nat n | None => 0 end.
-Definition add (x : elt) (n : nat) (s : t) : t := 
-  if eq_nat_dec n 0 then s else M.add x (Pos.of_nat (multiplicity x s + n)) s.
-Definition singleton x n := add x n empty.
-Definition remove (x : elt) (n : nat) (s : t) : t :=
-  if eq_nat_dec n 0 then s else
-  if le_lt_dec (multiplicity x s) n then M.remove x s else M.add x (Pos.of_nat (multiplicity x s - n)) s.
-Definition union (s s' : t) := M.fold (fun x n acc => add x (Pos.to_nat n) acc) s s'.
-Definition inter (s s' : t) :=
-  M.fold (fun x n acc => add x ((fun x n => min (multiplicity x s) (Pos.to_nat n)) x n) acc) s' empty.
-Definition diff (s s' : t) := M.fold (fun x n acc => add x (Pos.to_nat n - multiplicity x s') acc) s empty.
-Definition lub (s s' : t) := M.fold (fun x n acc => add x (Pos.to_nat n - multiplicity x s') acc) s s'.
-Definition equal (s s' : t) := M.equal Pos.eqb s s'.
-Definition subset s s' := is_empty (diff s s').
-Definition fold {A} f (s : t) := @M.fold positive A (fun x y => f x (Pos.to_nat y)) s.
-Definition for_all f (s : t) := M.fold (fun x n b => b && f x (Pos.to_nat n)) s true.
-Definition exists_ f (s : t) := M.fold (fun x n b => b || f x (Pos.to_nat n)) s false.
-Definition nfilter f (s : t) :=
-  M.fold (fun x n acc => if f x (Pos.to_nat n) : bool then add x (Pos.to_nat n) acc else acc) s empty.
-Definition filter f (s : t) := nfilter (fun x _ => f x) s.
-Definition npartition f (s : t) :=
-  M.fold (fun x n acc => if f x (Pos.to_nat n) : bool then (add x (Pos.to_nat n) (fst acc), snd acc)
-                                               else (fst acc, add x (Pos.to_nat n) (snd acc))) s (empty,empty).
-Definition partition f (s : t) := npartition (fun x _ => f x) s.
-Definition cardinal (s : t) := M.fold (fun _ n acc => Pos.to_nat n + acc) s 0.
-Definition size (s : t) := M.fold (fun _ _ n => S n) s 0.
-Definition elements (s : t) := List.map (fun xy => (fst xy, Pos.to_nat (snd xy))) (M.bindings s).
-Definition support (s : t) := M.fold (fun x _ l => cons x l) s nil.
-Definition choose (s : t) := M.fold (fun x _ _ => Some x) s None.
-
-Definition In := fun x s => multiplicity x s > 0.
-Definition eq s s' := forall x, multiplicity x s = multiplicity x s'.
-Definition Subset s s' := forall x, multiplicity x s <= multiplicity x s'.
-Definition For_all (P : elt -> nat -> Prop) s := forall x, In x s -> P x (multiplicity x s).
-Definition Exists (P : elt -> nat -> Prop) s := exists x, In x s /\ P x (multiplicity x s).
-
-Global Notation "s  [=]  t" := (eq s t) (at level 70, no associativity).
-Global Notation "s  [c=]  t" := (Subset s t) (at level 70, no associativity).
-
-Lemma eq_Meq : forall s s', s [=] s' <-> M.Equal s s'.
-Proof.
-intros s s'. unfold eq, multiplicity, M.Equal. split; intros Heq x.
-+ specialize (Heq x). destruct (M.find x s), (M.find x s').
-  - apply Pos2Nat.inj in Heq. now subst.
-  - assert (Hpos := Pos2Nat.is_pos p). omega.
-  - assert (Hpos := Pos2Nat.is_pos p). omega.
-  - reflexivity.
-+ now rewrite Heq.
-Qed.
-
-Instance multiplicity_compat : Proper (E.eq ==> eq ==> Logic.eq) multiplicity.
-Proof.
-intros x y Hxy s s' Hs. rewrite eq_Meq in Hs. unfold multiplicity. now rewrite (Mfind_compat _ _ Hxy _ _ Hs).
-Qed.
-
-Global Instance eq_equiv : Equivalence eq.
-Proof. split; try easy. intros x y z Hxy Hyz a. now rewrite Hxy, Hyz. Qed.
-(** [eq] is obviously an equivalence, for subtyping only. *)
-
-Instance In_compat : Proper (E.eq ==> eq ==> iff) In.
-Proof. intros x y Hxy s s' ?. unfold In. now rewrite H, Hxy. Qed.
-
-Theorem In_dec : forall x s, {In x s} + {~In x s}.
-Proof. unfold In. intros. apply gt_dec. Qed.
-
-Lemma In_MIn : forall x s, In x s <-> M.In x s.
+Lemma In_MIn : forall x s, FMapInterface.In x s <-> s[x] > 0.
 Proof.
 intros x s. split; intro H.
-- exists (Pos.of_nat (multiplicity x s)). rewrite <- M.find_spec. unfold In, multiplicity in *.
-  destruct (M.find x s). now rewrite Pos2Nat.id. now inversion H.
-- destruct H as [n Hn]. rewrite <- M.find_spec in Hn. unfold In, multiplicity. rewrite Hn. now apply Pos2Nat.is_pos.
+- destruct H as [n Hn]. rewrite find_mapsto_iff in Hn. simpl.
+  unfold multiplicity. rewrite Hn. now apply Pos2Nat.is_pos.
+- exists (Pos.of_nat (multiplicity x s)). rewrite find_mapsto_iff. simpl in *. unfold multiplicity in *.
+  destruct (find x s). now rewrite Pos2Nat.id. now inversion H.
 Qed.
 
-Lemma Mequal_Mequivb_equiv : forall s s' : M.t positive, M.Equal s s' <-> M.Equivb Pos.eqb s s'.
+Lemma Mequal_Mequivb_equiv : forall s s', Equal s s' <-> Equivb Pos.eqb s s'.
 Proof.
 intros s s'. split.
 + intro Heq. split.
   - intro x. split; intros [e Hin]; exists e.
-      now rewrite <- M.find_spec, <- Heq, M.find_spec.
-      now rewrite <- M.find_spec, Heq, M.find_spec.
-  - intros x e e' He He'. rewrite <- M.find_spec in *.
+      now rewrite find_mapsto_iff, <- Heq, <- find_mapsto_iff.
+      now rewrite find_mapsto_iff, Heq, <- find_mapsto_iff.
+  - intros x e e' He He'. rewrite find_mapsto_iff in He, He'.
     rewrite Heq in He. rewrite He in He'. inversion_clear He'. unfold Cmp. now apply Pos.eqb_refl.
 + intros [Heq1 Heq2] x.
-  destruct (M.find x s) as [e |] eqn:Hfind, (M.find x s') as [e' |] eqn:Hfind'.
-  - f_equal. apply Pos.eqb_eq. apply (Heq2 x); now rewrite <- M.find_spec.
-  - assert (Habs : M.In x s'). { rewrite <- Heq1. exists e. now rewrite <- M.find_spec. }
-    destruct Habs as [e' Habs]. rewrite <- M.find_spec, Hfind' in Habs. discriminate Habs.
-  - assert (Habs : M.In x s). { rewrite Heq1. exists e'. now rewrite <- M.find_spec. }
-    destruct Habs as [e Habs]. rewrite <- M.find_spec, Hfind in Habs. discriminate Habs.
+  destruct (find x s) as [e |] eqn:Hfind, (find x s') as [e' |] eqn:Hfind'.
+  - f_equal. apply Pos.eqb_eq. apply (Heq2 x); now rewrite find_mapsto_iff.
+  - assert (Habs : FMapInterface.In x s'). { rewrite <- Heq1. exists e. now rewrite find_mapsto_iff. }
+    destruct Habs as [e' Habs]. rewrite find_mapsto_iff, Hfind' in Habs. discriminate Habs.
+  - assert (Habs : FMapInterface.In x s). { rewrite Heq1. exists e'. now rewrite find_mapsto_iff. }
+    destruct Habs as [e Habs]. rewrite find_mapsto_iff, Hfind in Habs. discriminate Habs.
   - reflexivity.
 Qed.
 
-Lemma multiplicity_find_in : forall x s, In x s -> M.find x s = Some (Pos.of_nat (multiplicity x s)).
+Lemma multiplicity_out : forall x m, m[x] = 0 <-> find x m = None.
 Proof.
-intros x s Hin. unfold In, multiplicity in *. destruct (M.find x s) eqn:Hfind.
-- now rewrite Pos2Nat.id.
-- now inversion Hin.
-Qed.
-
-Lemma multiplicity_out : forall x s, multiplicity x s = 0 <-> M.find x s = None.
-Proof.
-unfold multiplicity. intros x s. split; intro Hs.
-+ destruct (M.find x s).
-  - elim (lt_irrefl 0). rewrite <- Hs at 2. now apply Pos2Nat.is_pos.
+simpl. unfold multiplicity. intros x m. split; intro Hm.
++ destruct (find x m) eqn:Hfind.
+  - elim (lt_irrefl 0). rewrite <- Hm at 2. now apply Pos2Nat.is_pos.
   - reflexivity.
-+ now rewrite Hs.
++ now rewrite Hm.
 Qed.
 
-Lemma equal_spec : forall s s', equal s s' = true <-> s[=]s'.
+(** **  Specifications of operations  **)
+
+Instance multiplicity_spec : MultiplicitySpec elt _.
 Proof.
-intros s s'. unfold equal. simpl. destruct (M.equal Pos.eqb s s') eqn:Heq.
-+ split; intro H; trivial || clear H. rewrite M.equal_spec, <- Mequal_Mequivb_equiv in Heq.
-  unfold eq, multiplicity. intro. now rewrite Heq.
-+ split; intro Habs; try discriminate Habs. exfalso.
-  assert (Hneq : ~M.Equivb Pos.eqb s s').
-  { intro Habs'. rewrite <- M.equal_spec, Heq in Habs'. discriminate Habs'. }
-  rewrite <- Mequal_Mequivb_equiv in Hneq. apply Hneq. intro x.
-  unfold eq, multiplicity in Habs. specialize (Habs x). simpl in Habs.
-  destruct (M.find x s) eqn:Hin1, (M.find x s') eqn:Hin2.
-  - f_equal. now apply Pos2Nat.inj.
-  - elim (lt_irrefl 0). rewrite <- Habs at 2. now apply Pos2Nat.is_pos.
-  - elim (lt_irrefl 0). rewrite Habs at 2. now apply Pos2Nat.is_pos.
-  - reflexivity.
+split.
+intros x y Hxy m m' Hm. rewrite Hm. simpl. unfold multiplicity.
+assert (Heq : find x m' = find y m') by now apply find_m.
+now rewrite Heq.
 Qed.
 
-Corollary eq_dec : forall s s' : t, {s [=] s'} + {~s [=] s'}.
+Instance empty_full_spec : EmptySpec elt _.
+Proof.
+split. intro x. simpl. unfold multiplicity, empty. simpl.
+destruct (find x (FMapInterface.empty positive)) eqn:Hin.
+- rewrite (empty_o positive x) in Hin. discriminate Hin.
+- reflexivity.
+Qed.
+
+Instance singleton_spec : SingletonSpec elt _.
+Proof. split.
++ intros x n. unfold singleton, add. simpl. destruct (Nat.eq_dec n 0).
+  - subst n. unfold multiplicity. now rewrite empty_o.
+  - unfold multiplicity. rewrite add_eq_o, Nat2Pos.id; trivial; reflexivity.
++ intros x y n Heq. unfold singleton, add. simpl. destruct (Nat.eq_dec n 0).
+  - subst n. unfold multiplicity. now rewrite empty_o.
+  - unfold multiplicity. rewrite add_neq_o, empty_o; reflexivity || now symmetry.
+Qed.
+
+Instance add_spec : AddSpec elt _.
+Proof. split.
++ intros x n s. unfold add. simpl. unfold m_add. destruct (Nat.eq_dec n 0). omega.
+  unfold multiplicity at 1. rewrite add_eq_o, Nat2Pos.id; reflexivity || omega.
++ intros x y n s Hyx. unfold add. simpl. unfold m_add. destruct (Nat.eq_dec n 0); trivial; [].
+  unfold multiplicity at 1 3. rewrite add_neq_o; reflexivity || now symmetry.
+Qed.
+
+Instance remove_spec : RemoveSpec elt _.
+Proof. split.
++ intros x n s. unfold remove. simpl. destruct (Nat.eq_dec n 0). omega.
+  destruct (le_lt_dec (multiplicity x s) n) as [Hle | Hlt]; unfold multiplicity at 1; simpl.
+  - rewrite remove_eq_o; reflexivity || omega.
+  - rewrite add_eq_o, Nat2Pos.id; reflexivity || omega.
++ intros x y n s Hyx. unfold remove. simpl. destruct (Nat.eq_dec n 0); trivial.
+  destruct (le_lt_dec (multiplicity x s) n) as [Hle | Hlt]; unfold multiplicity at 1; simpl.
+  - rewrite remove_neq_o; reflexivity || now symmetry.
+  - rewrite add_neq_o; reflexivity || now symmetry.
+Qed.
+
+Instance binary_spec :  BinarySpec elt _.
+Proof. split.
+* intros x s s'. unfold union. simpl. destruct (find x s) eqn:Hin.
+  - unfold multiplicity at 2. rewrite Hin. erewrite fold_add; eauto. now repeat intro.
+  - unfold multiplicity at 2. rewrite Hin. erewrite fold_add_out; eauto.
+    intros [n Habs]. now rewrite find_mapsto_iff, Hin in Habs.
+* intros x s s'. unfold inter. simpl. destruct (find x s') eqn:Hin.
+  + rewrite (fold_add (fun x n => min (multiplicity x s) n) x p s' (FMapInterface.empty _)); trivial.
+    - unfold multiplicity at 2 4. now rewrite empty_o, Hin, plus_0_r.
+    - intros ? ? Heq ? ? ?. simpl. subst. now rewrite Heq.
+  + rewrite fold_add_out.
+    - unfold multiplicity at 3. rewrite Hin, Min.min_0_r. unfold multiplicity. now rewrite empty_o.
+    - intros [n Habs]. now rewrite find_mapsto_iff, Hin in Habs.
+* intros x s s'. unfold diff. simpl. destruct (find x s) eqn:Hin.
+  + rewrite (fold_add (fun x n => n - multiplicity x s') x p s (FMapInterface.empty _)); trivial.
+    - unfold multiplicity at 2 3. now rewrite empty_o, Hin, plus_0_r.
+    - intros ? ? Heq ? ? ?. subst. now rewrite Heq.
+  + rewrite fold_add_out.
+    - unfold multiplicity at 2. rewrite Hin. simpl. unfold multiplicity. now rewrite empty_o.
+    - intros [n Habs]. now rewrite find_mapsto_iff, Hin in Habs.
+* intros x s s'. unfold lub. simpl.
+  replace (max (multiplicity x s) (multiplicity x s'))
+    with (multiplicity x s - multiplicity x s'  + multiplicity x s') by (apply Max.max_case_strong; omega).
+  destruct (find x s) eqn:Hin.
+  + erewrite (fold_add); eauto.
+    - unfold multiplicity at 3. now rewrite Hin.
+    - intros ? ? Heq ? ? ?. subst. now rewrite Heq.
+  + rewrite fold_add_out.
+    - unfold multiplicity at 2. now rewrite Hin.
+    - intros [n Habs]. now rewrite find_mapsto_iff, Hin in Habs.
+Qed.
+
+Instance fold_full_spec : FoldSpec elt _.
+Proof. split.
+* intros A i f s. unfold fold, elements. simpl. unfold m_fold.
+  now rewrite FMapInterface.fold_1, fold_left_map.
+* intros A eqA HeqA f Hf Hfcomm s1 s2 Hs x y Hxy.
+  unfold fold. simpl. unfold m_fold. do 2 rewrite FMapInterface.fold_1.
+  rewrite fold_left_symmetry_PermutationA.
+  + reflexivity.
+  + apply eq_key_elt_Equivalence.
+  + assumption.
+  + repeat intro. now apply Hf; try rewrite H1 || rewrite H0.
+  + intros. apply Hfcomm.
+  + apply NoDupA_equivlistA_PermutationA.
+    - autoclass.
+    - eapply NoDupA_strengthen; apply eq_key_eq_key_elt_subrelation || apply elements_3.
+    - eapply NoDupA_strengthen; apply eq_key_eq_key_elt_subrelation || apply elements_3.
+    - clear -Hs MapSpec. intros [x n].
+      setoid_rewrite <- @elements_mapsto_iff; trivial; []. setoid_rewrite @find_mapsto_iff; trivial; [].
+      specialize (Hs x). cbn in Hs. unfold multiplicity in Hs.
+      destruct (find x s1), (find x s2);
+      solve [ apply Pos2Nat.inj in Hs; subst; reflexivity
+            | elim (lt_irrefl 0); rewrite Hs at 2 || rewrite <- Hs at 2; apply Pos2Nat.is_pos
+            | split; intro; discriminate ].
+  + assumption.
+Qed.
+
+Instance test_spec : TestSpec elt _.
+Proof.
+assert (His_empty_spec : forall s, is_empty s = true <-> s == empty).
+{ intros s. unfold is_empty. simpl. split; intro H.
+  + rewrite <- is_empty_iff in H. intros x. unfold multiplicity. rewrite empty_o.
+    destruct (find x s) eqn:Hin; trivial. rewrite <- find_mapsto_iff in Hin. now apply H in Hin.
+  + rewrite <- is_empty_iff. intros x n Habs.
+    rewrite find_mapsto_iff in Habs. specialize (H x).
+    unfold multiplicity in H. rewrite Habs, empty_o in H.
+    apply (lt_irrefl 0). rewrite <- H at 2. apply Pos2Nat.is_pos. }
+split; trivial.
+* intros s s'. unfold equal. simpl.
+  destruct (FMapInterface.equal Pos.eqb s s') eqn:Heq.
+  + split; intro H; trivial || clear H. rewrite <- equal_iff, <- Mequal_Mequivb_equiv in Heq.
+    unfold multiplicity. intro. now rewrite Heq.
+  + split; intro Habs; try discriminate Habs. exfalso.
+    assert (Hneq : ~FMapInterface.Equivb Pos.eqb s s').
+    { intro Habs'. rewrite equal_iff, Heq in Habs'. discriminate Habs'. }
+    rewrite <- Mequal_Mequivb_equiv in Hneq. apply Hneq. intro x.
+    unfold multiplicity in Habs. specialize (Habs x). simpl in Habs.
+    destruct (find x s) eqn:Hin1, (find x s') eqn:Hin2.
+    - f_equal. now apply Pos2Nat.inj.
+    - elim (lt_irrefl 0). rewrite <- Habs at 2. now apply Pos2Nat.is_pos.
+    - elim (lt_irrefl 0). rewrite Habs at 2. now apply Pos2Nat.is_pos.
+    - reflexivity.
+* intros s s'. unfold subset. simpl.
+  cbn in His_empty_spec. rewrite His_empty_spec. clear His_empty_spec.
+  unfold multiplicity at 3. setoid_rewrite empty_o.
+  split; intro Hle.
+  + intro x. destruct (find x s) eqn:Hin.
+    - cut (s[x] - s'[x] = 0). omega. rewrite <- diff_spec. simpl.
+      erewrite fold_add; eauto.
+      ++ unfold multiplicity at 2. rewrite empty_o, plus_0_r.
+         specialize (Hle x). erewrite fold_add in Hle; eauto.
+         -- unfold multiplicity at 2 in Hle. now rewrite empty_o, plus_0_r in Hle.
+         -- intros ? ? Heq ? ? ?. subst. now rewrite Heq.
+      ++ intros ? ? Heq ? ? ?. subst. now rewrite Heq.
+    - simpl. unfold multiplicity at 1. rewrite Hin. omega.
+  + intro x. destruct (find x s) eqn:Hin.
+    - erewrite fold_add; eauto.
+      -- unfold multiplicity at 2. rewrite empty_o, plus_0_r.
+         specialize (Hle x). simpl in Hle. unfold multiplicity at 1 in Hle. rewrite Hin in Hle. omega.
+      -- intros ? ? Heq ? ? ?. subst. now rewrite Heq.
+    - erewrite fold_add_out; eauto.
+      -- unfold multiplicity. now rewrite empty_o.
+      -- intros [n Habs]. now rewrite find_mapsto_iff, Hin in Habs.
+Qed.
+
+Corollary eq_dec : forall s s', {s == s'} + {s =/= s'}.
 Proof.
 intros s s'. destruct (equal s s') eqn:Heq.
 - left. now rewrite <- equal_spec.
-- right. rewrite <- equal_spec. rewrite Heq. discriminate.
+- right. intro H. revert H. rewrite <- equal_spec. rewrite Heq. discriminate.
 Qed.
 
-Lemma empty_spec : forall x, multiplicity x empty = 0.
-Proof.
-intro x. unfold multiplicity, empty.
-destruct (M.find x M.empty) eqn:Hin.
-- rewrite (M.empty_spec positive x) in Hin. discriminate Hin.
-- reflexivity.
+Instance elements_full_spec : ElementsSpec elt _.
+Proof. split.
+* intros x n s. unfold elements. simpl. rewrite InA_map_iff; [split; intro H |..].
+  + destruct H as [[y m] [[Heq1 Heq2] Hin]]. hnf in Heq1, Heq2. cbn in Heq1, Heq2. subst.
+    rewrite <- elements_mapsto_iff, find_mapsto_iff in Hin.
+    unfold multiplicity. rewrite <- Heq1, Hin. split; trivial. apply Pos2Nat.is_pos.
+  + exists (x, Pos.of_nat n). destruct H as [H1 H2]. simpl in *. split.
+    - split; hnf; simpl. reflexivity. apply Nat2Pos.id. omega.
+    - rewrite <- elements_mapsto_iff, find_mapsto_iff. subst. unfold multiplicity in *.
+      destruct (find x s). now rewrite Pos2Nat.id. omega.
+  + autoclass.
+  + autoclass.
+  + clear. intros [] [] []. intros. split; simpl in *. assumption. now subst.
+* intro s. unfold elements. simpl. rewrite NoDupA_inj_map;
+apply elements_3 || autoclass || (intros [] [] ?; assumption).
 Qed.
 
-Lemma is_empty_spec : forall s, is_empty s = true <-> s [=] empty.
-Proof.
-intros s. unfold is_empty. split; intro H.
-+ rewrite M.is_empty_spec in H. intros x. rewrite empty_spec.
-  unfold multiplicity. now rewrite H.
-+ rewrite M.is_empty_spec. intro x. rewrite eq_Meq in H. rewrite H. apply M.empty_spec.
-Qed.
-
-Corollary is_empty_multiplicity : forall x s, is_empty s = true -> multiplicity x s = 0.
-Proof.
-intros x s Hs. unfold multiplicity. destruct (M.find x s) eqn:Hin; trivial.
-rewrite is_empty_spec in Hs. rewrite eq_Meq in Hs. rewrite Hs, M.empty_spec in Hin. discriminate.
-Qed.
-
-Lemma add_same : forall x n s, multiplicity x (add x n s) = multiplicity x s + n.
-Proof.
-intros x n s. unfold add. destruct (eq_nat_dec n 0). omega.
-unfold multiplicity at 1. simpl.
-rewrite (M.add_spec1 s x (Pos.of_nat (multiplicity x s + n))).
-rewrite Nat2Pos.id. reflexivity. omega.
-Qed.
-
-Lemma add_other : forall x y n s, ~E.eq y x -> multiplicity y (add x n s) = multiplicity y s.
-Proof.
-intros x y n s Hyx. unfold add. destruct (eq_nat_dec n 0); trivial. unfold multiplicity at 1 3.
-rewrite (M.add_spec2 s (Pos.of_nat (multiplicity x s + n))). reflexivity. now intro; apply Hyx.
-Qed.
-
-Lemma remove_same : forall x n s, multiplicity x (remove x n s) = multiplicity x s - n.
-Proof.
-intros x n s. unfold remove. destruct (eq_nat_dec n 0). omega.
-destruct (le_lt_dec (multiplicity x s) n) as [Hle | Hlt]; unfold multiplicity at 1; simpl.
-- rewrite M.remove_spec1. omega.
-- rewrite M.add_spec1. rewrite Nat2Pos.id. reflexivity. omega.
-Qed.
-
-Lemma remove_other : forall x y n s, ~E.eq y x -> multiplicity y (remove x n s) = multiplicity y s.
-Proof.
-intros x y n s Hyx. unfold remove. destruct (eq_nat_dec n 0); trivial.
-assert (Hxy : ~E.eq x y) by (intro; now apply Hyx).
-destruct (le_lt_dec (multiplicity x s) n) as [Hle | Hlt]; unfold multiplicity at 1; simpl.
-- now rewrite M.remove_spec2.
-- now rewrite M.add_spec2.
-Qed.
-
-Lemma singleton_same : forall x n, multiplicity x (singleton x n) = n.
-Proof.
-intros x n. unfold singleton, add. destruct (eq_nat_dec n 0).
-+ subst n. apply empty_spec.
-+ rewrite empty_spec. simpl. unfold multiplicity. rewrite M.add_spec1. now apply Nat2Pos.id.
-Qed.
-
-Lemma singleton_other : forall x y n, ~E.eq y x -> multiplicity y (singleton x n) = 0.
-Proof.
-intros x y n Heq. unfold singleton, add. destruct (eq_nat_dec n 0).
-+ subst n. apply empty_spec.
-+ rewrite empty_spec. simpl. unfold multiplicity. rewrite M.add_spec2, M.empty_spec; trivial. intro; now apply Heq.
-Qed.
-
-Lemma fold_add_out_list : forall f x n l s, ~InA (@M.eq_key positive) (x, n) l -> NoDupA (@M.eq_key _) l ->
-  multiplicity x (fold_left (fun acc xn => add (fst xn) (f (fst xn) (snd xn)) acc) l s) = multiplicity x s.
-Proof.
-intros f x n l s Hin Hdup. revert s. induction l as [| [y m] l]; intro s; simpl.
-- reflexivity.
-- rewrite IHl. apply add_other. intro Habs. apply Hin. left. compute. auto. auto. now inversion_clear Hdup.
-Qed.
-
-Lemma fold_add_out : forall f x (s s' : t), ~M.In x s -> 
-  multiplicity x (M.fold (fun x n acc => add x (f x n) acc) s s') = multiplicity x s'.
-Proof.
-intros f x s s' Hin. rewrite M.fold_spec.
-assert (Hs : forall n, ~(InA (@M.eq_key_elt _) (x, n) (M.bindings s))).
-{ intros n Habs. apply Hin. exists n. now rewrite <- M.bindings_spec1. }
-revert s'. induction (M.bindings s) as [| [y m] l]; intro s'; simpl.
-+ reflexivity.
-+ assert ( Hxy : ~E.eq x y). { intro Habs. apply (Hs m). left. now split. }
-  rewrite IHl.
-  - apply add_other. now auto.
-  - intros n Habs. apply (Hs n). now right.
-Qed.
-
-Notation compatb := (Proper (E.eq ==> Logic.eq ==> Logic.eq)) (only parsing).
-
-Lemma fold_add : forall f x (s s' : t), compatb f -> M.In x s -> 
-  multiplicity x (M.fold (fun x n acc => add x (f x (Pos.to_nat n)) acc) s s')
-  = f x (multiplicity x s) + multiplicity x s'.
-Proof.
-intros f x s s' Hf [n Hin]. rewrite M.fold_spec.
-assert (Hs : InA (@M.eq_key_elt positive) (x, n) (M.bindings s)) by now rewrite M.bindings_spec1.
-assert (Hdup := M.bindings_spec2w s).
-revert s'. induction (M.bindings s) as [| [y m] l]; intro s'; simpl; [now inversion Hs |].
-destruct (Meq_dec (x, n) (y, m)) as [[H1 H2] | Hneq]; simpl in *; try subst m.
-* transitivity (multiplicity x (add y (f y (Pos.to_nat n)) s')).
-  + rewrite (fold_add_out_list (fun x y => f x (Pos.to_nat y)) x n).
-    - reflexivity.
-    - inversion_clear Hdup. clear -H H1. intro Habs. apply H. revert Habs. apply InA_eqA; trivial. refine _.
-    - now inversion_clear Hdup.
-  + rewrite H1, add_same, plus_comm. f_equal. unfold multiplicity.
-    rewrite H1, <- M.find_spec in Hin. now rewrite Hin.
-* rewrite IHl.
-  + f_equal. apply add_other. intro Habs. apply Hneq. compute. split. now auto.
-    apply (NoDup_pair_In _ x y n m ((y, m) :: l)); trivial. left. compute. now auto.
-  + inversion_clear Hs. contradiction. assumption.
-  + now inversion_clear Hdup.
-Qed.
-
-Lemma union_spec : forall x s s', multiplicity x (union s s') = multiplicity x s + multiplicity x s'.
-Proof.
-intros x s s'. unfold union. destruct (M.find x s) eqn:Hin.
-- apply (fold_add (fun x n => n)). now intros until 2. exists p. now rewrite <- M.find_spec.
-- unfold multiplicity at 2. rewrite Hin. simpl. apply fold_add_out.
-  intros [n Habs]. now rewrite <- M.find_spec, Hin in Habs.
-Qed.
-
-Lemma inter_spec : forall x s s', multiplicity x (inter s s') = min (multiplicity x s) (multiplicity x s').
-Proof.
-intros x s s'. unfold inter. destruct (M.find x s') eqn:Hin.
-+ rewrite (fold_add (fun x n => min (multiplicity x s) n) x s' empty).
-  - rewrite (empty_spec x). now rewrite plus_0_r.
-  - intros ? ? Heq ? ? ?. simpl. subst. now rewrite Heq.
-  - exists p. now rewrite <- M.find_spec.
-+ rewrite fold_add_out.
-  - unfold multiplicity at 3. rewrite Hin. rewrite Min.min_0_r. now apply empty_spec.
-  - intros [n Habs]. now rewrite <- M.find_spec, Hin in Habs.
-Qed.
-
-Lemma diff_spec : forall x s s', multiplicity x (diff s s') = multiplicity x s - multiplicity x s'.
-Proof.
-intros x s s'. unfold diff. destruct (M.find x s) eqn:Hin.
-+ rewrite (fold_add (fun x n => n - multiplicity x s') x s empty).
-  - rewrite empty_spec. now rewrite plus_0_r.
-  - intros ? ? Heq ? ? ?. subst. now rewrite Heq.
-  - exists p. now rewrite <- M.find_spec.
-+ rewrite fold_add_out.
-  - unfold multiplicity at 2. rewrite Hin. simpl. now apply empty_spec.
-  - intros [n Habs]. now rewrite <- M.find_spec, Hin in Habs.
-Qed.
-
-Lemma lub_spec : forall x s s', multiplicity x (lub s s') = max (multiplicity x s) (multiplicity x s').
-Proof.
-Proof.
-intros x s s'. unfold lub.
-replace (max (multiplicity x s) (multiplicity x s'))
-  with (multiplicity x s - multiplicity x s'  + multiplicity x s') by (apply Max.max_case_strong; omega).
-destruct (M.find x s) eqn:Hin.
-+ apply (fold_add (fun x n => n - multiplicity x s')).
-  - intros ? ? Heq ? ? ?. subst. now rewrite Heq.
-  - exists p. now rewrite <- M.find_spec.
-+ rewrite fold_add_out.
-  - unfold multiplicity at 2. rewrite Hin. simpl. reflexivity.
-  - intros [n Habs]. now rewrite <- M.find_spec, Hin in Habs.
-Qed.
-
-Lemma subset_spec : forall s s', subset s s' = true <-> s [c=] s'.
-Proof.
-intros s s'. split; intro Hle.
-- intro x. apply (is_empty_multiplicity x) in Hle. rewrite diff_spec in Hle. omega.
-- unfold subset. rewrite is_empty_spec. intro x. unfold In. rewrite diff_spec.
-  specialize (Hle x). rewrite empty_spec. omega.
-Qed.
-
-Lemma fold_spec : forall (A : Type) s (i : A) (f : elt -> nat -> A -> A),
-    fold f s i = fold_left (fun acc xn => f (fst xn) (snd xn) acc) (elements s) i.
-Proof. intros A i f s. unfold fold, elements. now rewrite M.fold_spec, fold_left_map. Qed.
-
-Lemma cardinal_spec : forall s, cardinal s = fold (fun x n acc => n + acc) s 0.
-Proof. intro. unfold cardinal. rewrite fold_spec. unfold elements. now rewrite fold_left_map, M.fold_spec. Qed.
-
-Lemma size_spec : forall s, size s = length (support s).
-Proof.
-intro. unfold size, support. now rewrite M.fold_spec, fold_left_length, M.fold_spec, fold_left_cons_length.
-Qed.
-
-
-Lemma Melements_multiplicity : forall s x n,
-  InA (@M.eq_key_elt _) (x, n) (M.bindings s)
-  <-> multiplicity x s = Pos.to_nat n /\ Pos.to_nat n > 0.
-Proof.
-intros s x n. split; intro H.
-+ apply M.bindings_spec1, M.find_spec in H. unfold multiplicity.
-  rewrite H. split. reflexivity. apply Pos2Nat.is_pos.
-+ destruct H as [H1 H2]. unfold multiplicity in H1. destruct (M.find x s) eqn:Hin.
-  - rewrite M.bindings_spec1, <- M.find_spec. rewrite Hin. f_equal. now apply Pos2Nat.inj.
-  - rewrite  <- H1 in H2. inversion H2.
-Qed.
-
-Corollary elements_spec : forall x n s,
-  InA eq_pair (x, n) (elements s) <-> multiplicity x s = n /\ n > 0.
-Proof.
-intros x n s. unfold elements. rewrite InA_map_iff.
-split; intro H.
-+ destruct H as [[y m] [[Heq1 Heq2] Hin]]. rewrite Melements_multiplicity in Hin.
-  hnf in Heq1, Heq2. simpl in *. subst n. now rewrite <- Heq1.
-+ exists (x, Pos.of_nat n). destruct H as [H1 H2]. simpl in *. split.
-  - split; hnf; simpl. reflexivity. apply Nat2Pos.id. omega.
-  - rewrite Melements_multiplicity. simpl. rewrite H1. rewrite Nat2Pos.id. now split. omega.
-+ apply Meq_equiv.
-+ apply Meq_equiv.
-+ clear. intros [] [] []. intros. split; simpl in *. assumption. now subst.
-Qed.
-
-Lemma elements_NoDupA : forall s, NoDupA (@M.eq_key _) (elements s).
-Proof.
-intro s. unfold elements. rewrite NoDupA_inj_map; 
-apply M.bindings_spec2w || apply Meq_key_equiv || (intros [] [] ?; assumption).
-Qed.
-
-Lemma support_elements_aux : forall x l1 l2, NoDupA (@M.eq_key _) (l1 ++ l2) -> 
-  ((InA E.eq x (fold_left (fun acc xn => fst xn :: acc) l1 (map (@fst _ _) l2)) <->
-  exists n, InA eq_pair (x, n) (map (fun xn => (fst xn, Pos.to_nat (snd xn))) (l1 ++ l2)))).
+Lemma support_elements_aux : forall x l1 l2, NoDupA eq_key (l1 ++ l2) -> 
+  ((InA equiv x (fold_left (fun acc xn => fst xn :: acc) l1 (List.map (@fst _ positive) l2)) <->
+  exists n, InA eq_key_elt (x, n) (List.map (fun xn => (fst xn, snd xn)) (l1 ++ l2)))).
 Proof.
 intros x l1. induction l1; simpl; intros l2 Hdup.
 * split; intro H.
   + induction l2.
     - now inversion H.
     - destruct a as [y m]. inversion_clear H.
-        exists (Pos.to_nat m). left. now split.
+        exists m. left. now split.
         apply IHl2 in H0. destruct H0 as [n Hn]. exists n. simpl. now right. now inversion_clear Hdup.
   + destruct H as [n Hn]. induction l2; simpl.
     - now inversion Hn.
@@ -513,8 +478,8 @@ intros x l1. induction l1; simpl; intros l2 Hdup.
         left. now destruct H1.
         right. now apply IHl2.
 * destruct a as [y m]. simpl. split; intro H.
-  + destruct (E.eq_dec x y). exists (Pos.to_nat m). left. now split.
-    change (y :: map (fst (B:=positive)) l2) with (map (fst (B:=positive)) ((y,m) :: l2)) in H.
+  + destruct (equiv_dec x y). exists m. left. now split.
+    change (y :: List.map (fst (B:=positive)) l2) with (List.map (fst (B:=positive)) ((y,m) :: l2)) in H.
     rewrite IHl1 in H.
     - destruct H as [p Hp]. exists p. rewrite map_app in *. rewrite InA_app_iff in Hp.
         simpl in Hp. destruct Hp.
@@ -523,179 +488,174 @@ intros x l1. induction l1; simpl; intros l2 Hdup.
              now left.
              right. rewrite InA_app_iff. now right.
     - rewrite NoDupA_swap_iff. assumption. refine _.
-  + change (y :: map (fst (B:=positive)) l2) with (map (fst (B:=positive)) ((y,m) :: l2)).
+  + change (y :: List.map (fst (B:=positive)) l2) with (List.map (fst (B:=positive)) ((y,m) :: l2)).
     rewrite IHl1. destruct H as [n Hn]. exists n. rewrite map_app, InA_app_iff. inversion_clear Hn.
     - right. now left.
     - rewrite map_app, InA_app_iff in H. destruct H. now left. now do 2 right.
-    - rewrite NoDupA_swap_iff. assumption. now apply Meq_key_equiv.
+    - rewrite NoDupA_swap_iff. assumption. autoclass.
 Qed.
 
-Lemma support_elements : forall x s, InA E.eq x (support s) <-> InA eq_pair (x, multiplicity x s) (elements s).
+Lemma support_elements : forall x s, InA equiv x (support s) <-> InA eq_pair (x, multiplicity x s) (elements s).
 Proof.
-intros x s. unfold support, elements. rewrite M.fold_spec.
-change nil with (map (@fst E.t nat) nil).
-rewrite (support_elements_aux x (M.bindings s) nil); rewrite app_nil_r; [split; intro H |].
+intros x s. unfold support, elements. simpl. rewrite fold_1.
+change nil with (List.map (@fst elt positive) nil).
+rewrite (support_elements_aux x (FMapInterface.elements s) nil); rewrite app_nil_r; [split; intro H |].
 + destruct H as [n Hn].
-  assert (n = multiplicity x s).
-  { rewrite (InA_map_iff (Meq_equiv _) eq_pair_equiv) in Hn.
-    - destruct Hn as [[y m] [[Heqx Heqn] Hin]]. rewrite Melements_multiplicity in Hin. 
-      hnf in *. simpl in *. subst. symmetry. destruct Hin. rewrite <- Heqx. assumption.
-    - intros [? ?] [? ?] Heq; simpl in *. hnf in Heq. destruct Heq; split; hnf; simpl in *; subst; auto. }
-  now subst n.
-+ now exists (multiplicity x s).
-+ apply M.bindings_spec2w.
+  rewrite (@InA_map_iff _ _ eq_key_elt) in Hn; try rewrite (@InA_map_iff _ _ eq_key_elt); autoclass;
+  try (now intros [? ?] [? ?] Heq; simpl in *; hnf in Heq; destruct Heq; split; hnf; simpl in *; subst; auto); [].
+  destruct Hn as [[y m] [[Heqx Heqn] Hin]]. exists (y, m). repeat split; eauto; try now hnf in *; cbn in *.
+  subst. rewrite <- elements_mapsto_iff, find_mapsto_iff in Hin. 
+  hnf in *. simpl in *. subst. unfold multiplicity.
+  rewrite find_m in Hin; eauto; try now intro; reflexivity. now rewrite Hin.
++ exists (Pos.of_nat (multiplicity x s)).
+  rewrite (@InA_map_iff _ _ eq_key_elt) in H; try rewrite (@InA_map_iff _ _ eq_key_elt); autoclass;
+  try (now intros [? ?] [? ?] Heq; simpl in *; hnf in Heq; destruct Heq; split; hnf; simpl in *; subst; auto); [].
+  destruct H as [[y m] [[Heqx Heqn] Hin]]. exists (y, m). repeat split; eauto; try now hnf in *; cbn in *.
+  subst. rewrite <- elements_mapsto_iff, find_mapsto_iff in Hin. 
+  hnf in *. simpl in *. subst. unfold multiplicity.
+  rewrite find_m in Hin; eauto; try now intro; reflexivity. now rewrite Hin, Pos2Nat.id.
++ apply elements_3.
 Qed.
-
-Corollary support_spec : forall x s, InA E.eq x (support s) <-> In x s.
-Proof. intros x s. rewrite support_elements. rewrite elements_spec. intuition. Qed.
 
 Lemma support_NoDupA_aux : forall A B (l1 : list (A*B)) l2,
-  fold_left (fun acc p => fst p :: acc) l1 l2 = rev (map (@fst _ _) l1) ++ l2.
+  fold_left (fun acc p => fst p :: acc) l1 l2 = rev (List.map (@fst _ _) l1) ++ l2.
 Proof.
 intros A B l1. induction l1; intro l2; simpl.
-  reflexivity.
-  rewrite IHl1. now rewrite <- app_assoc.
-Qed.
-
-Lemma support_NoDupA : forall s, NoDupA E.eq (support s).
-Proof.
-intro s. unfold support. rewrite M.fold_spec, support_NoDupA_aux, app_nil_r.
-apply NoDupA_rev. now auto with typeclass_instances.
-rewrite NoDupA_inj_map; (now apply M.bindings_spec2w) || (now auto with typeclass_instances) || (now intros ? ? ?).
-Qed.
-
-
-Lemma fold_nfilter_out_list : forall f x n l s, ~InA (@M.eq_key positive) (x, n) l -> NoDupA (@M.eq_key _) l ->
-  multiplicity x (fold_left (fun acc xn => if f (fst xn) (snd xn) : bool
-                                           then add (fst xn) (Pos.to_nat (snd xn)) acc else acc) l s)
-  = multiplicity x s.
-Proof.
-intros f x n l s Hin Hdup. revert s. induction l as [| [y m] l]; intro s; simpl.
-  reflexivity.
-  rewrite IHl.
-    destruct (f y m). apply add_other. intro Habs. apply Hin. left. compute. auto. auto.
-    intro Habs. apply Hin. now right.
-    now inversion_clear Hdup.
-Qed.
-
-Lemma nfilter_spec_In : forall f s s' x, compatb f -> In x s ->
-  multiplicity x
-    (M.fold
-       (fun (x0 : M.key) (n : positive) (acc : t) =>
-        if f x0 (Pos.to_nat n) : bool then add x0 (Pos.to_nat n) acc else acc) s s')
-  = if f x (multiplicity x s) then multiplicity x s + multiplicity x s' else multiplicity x s'.
-Proof.
-intros f s s' x Hf Hin. rewrite M.fold_spec. revert s'. unfold In in Hin.
-assert (Hs : InA (@M.eq_key_elt _) (x, multiplicity x s) (elements s)). { rewrite elements_spec. simpl. now split. }
-assert (Hdup : NoDupA (@M.eq_key _) (elements s)) by apply elements_NoDupA.
-unfold elements in Hs, Hdup.
-induction (M.bindings s); simpl; intro s'; simpl in Hs.
-* exfalso. rewrite <- InA_nil. apply Hs.
-* destruct a as [y m].
-  destruct (Meq_dec (x, Pos.of_nat (multiplicity x s)) (y, m)) as [Heq | Hneq].
-  + destruct Heq as [H1 H2]. simpl in H1, H2 |- *. rewrite H1 in *. subst m.
-    rewrite (fold_nfilter_out_list (fun x y => f x (Pos.to_nat y)) _ (Pos.of_nat (multiplicity y s))).
-    - rewrite Nat2Pos.id; try omega.
-      destruct (f y (multiplicity y s)) eqn:Htest.
-        rewrite add_same, H1. now apply plus_comm.
-        now rewrite H1.
-    - inversion_clear Hdup. intro Habs. apply H. rewrite InA_map_iff.
-        exists (y, Pos.of_nat (multiplicity y s)). split. reflexivity. eassumption.
-        apply Meq_key_equiv.
-        apply Meq_key_equiv.
-        clear. intros [] [] Hxy. now compute in *.
-    - inversion_clear Hdup. rewrite NoDupA_inj_map in H0.
-        eassumption.
-        now apply Meq_key_equiv.
-        now apply Meq_key_equiv.
-        now intros [] [].
-        now intros [] [].
-  + inversion_clear Hs.
-    - elim Hneq. destruct H. split. assumption. simpl in *. now rewrite H0, Pos2Nat.id.
-    - inversion_clear Hdup. assert (Hxy : ~E.eq x y).
-      { intro Habs. apply H0. now apply (eq_key_elt_eq_key_weak_In _ x y (multiplicity x s)). }
-      rewrite IHl; try assumption. simpl.
-      destruct (f x (multiplicity x s)), (f y (Pos.to_nat m));
-      reflexivity || rewrite add_other; reflexivity || now auto.
-Qed.
-
-Lemma nfilter_spec_out : forall f s s' x, ~In x s ->
-  multiplicity x
-    (M.fold
-       (fun (x0 : M.key) (n : positive) (acc : t) =>
-        if f x0 (Pos.to_nat n) : bool then add x0 (Pos.to_nat n) acc else acc) s s')
-  = multiplicity x s'.
-Proof.
-intros f s s' x Hin. rewrite M.fold_spec.
-assert (Hs : forall n, ~(InA (@M.eq_key_elt _) (x, n) (M.bindings s))).
-{ intros n Habs. apply Hin. rewrite M.bindings_spec1, <- M.find_spec in Habs.
-  unfold In, multiplicity. rewrite Habs. apply Pos2Nat.is_pos. }
-revert s'. induction (M.bindings s) as [| [y m] l]; intro s'; simpl.
-  reflexivity.
-  assert ( Hxy : ~E.eq x y). { intro Habs. apply (Hs m). left. now split. }
-  rewrite IHl. destruct (f y (Pos.to_nat m)). apply add_other. now auto. reflexivity.
-  intros n Habs. apply (Hs n). now right.
-Qed.
-
-Corollary nfilter_spec : forall f x s, compatb f ->
-    multiplicity x (nfilter f s) = if f x (multiplicity x s) then multiplicity x s else 0.
-Proof.
-intros f x s Hf. unfold nfilter.
-destruct (multiplicity x s) eqn:Hin.
-  rewrite nfilter_spec_out.
-    now destruct (f x 0); apply empty_spec.
-    unfold In. omega.
-  rewrite nfilter_spec_In.
-    now rewrite empty_spec, Hin, plus_0_r.
-    assumption.
-    unfold In. rewrite Hin. omega.
-Qed.
-
-
-Theorem filter_nfilter : forall f s, filter f s [=] nfilter (fun x _ => f x) s.
-Proof. now unfold filter. Qed.
-
-Corollary filter_spec : forall f x s, Proper (E.eq ==> Logic.eq) f ->
-    multiplicity x (filter f s) = if f x then multiplicity x s else 0.
-Proof.
-intros f x s Hf. rewrite filter_nfilter, nfilter_spec.
 - reflexivity.
-- repeat intro. now apply Hf.
+- rewrite IHl1. now rewrite <- app_assoc.
 Qed.
 
+Instance support_spec : SupportSpec elt _.
+Proof. split.
+* intros x s. rewrite support_elements. rewrite elements_spec. intuition.
+* intro s. unfold support. simpl. rewrite fold_1, support_NoDupA_aux, app_nil_r.
+  apply NoDupA_rev; autoclass; [].
+  rewrite NoDupA_inj_map; (now apply elements_3) || autoclass || (now intros ? ? ?).
+Qed.
 
-Lemma choose_spec_aux : forall x s o, ~M.In x s ->
-  fold_left (fun (_ : option M.key) (p : M.key * positive) => Some (fst p)) (M.bindings s) o = Some x ->
+Lemma choose_spec_aux : forall x s o, ~FMapInterface.In x s ->
+  fold_left (fun (_ : option elt) (p : elt * positive) => Some (fst p)) (FMapInterface.elements s) o = Some x ->
   o = Some x.
 Proof.
 intros x s o Hs.
-assert (Hs' : forall n, ~InA (@M.eq_key_elt _) (x, n) (M.bindings s)).
-{ intros n Habs. apply Hs. exists n. now apply M.bindings_spec1. } clear Hs.
-revert o. induction (M.bindings s); simpl; intros o Hin.
+assert (Hs' : forall n, ~InA eq_key_elt (x, n) (FMapInterface.elements s)).
+{ intros n Habs. apply Hs. exists n. now apply elements_2. } clear Hs.
+revert o. induction (FMapInterface.elements s); simpl; intros o Hin.
 + assumption.
 + apply IHl in Hin.
   - elim (Hs' (snd a)). left. split; simpl. now inversion Hin. reflexivity.
   - intros n Habs. apply (Hs' n). now right.
 Qed.
 
-Lemma choose_Some : forall x s, choose s = Some x -> In x s.
+Instance choose_spec : ChooseSpec elt _.
 Proof.
-intros x s Hin. destruct (In_dec x s). assumption. unfold choose in Hin.
-rewrite M.fold_spec in Hin. apply choose_spec_aux in Hin. now inversion Hin. now rewrite <- In_MIn.
+assert (Hchoose_Some : forall (x : elt) (s : multiset), choose s = Some x -> In x s).
+{ intros x s Hin. destruct (In_dec s x).
+  + unfold In. now rewrite <- In_MIn.
+  + unfold choose in Hin. simpl in Hin. rewrite fold_1 in Hin.
+    apply choose_spec_aux in Hin; trivial; discriminate. }
+split; trivial.
+* intros s. split; intro Hs.
+  + intro x. unfold choose in Hs. simpl in Hs. rewrite fold_1 in Hs. rewrite empty_spec. rewrite multiplicity_out.
+    destruct (find x s) eqn:Habs; trivial; [].
+    rewrite <- find_mapsto_iff in Habs. apply elements_1 in Habs. destruct (FMapInterface.elements s).
+    - now inversion Habs.
+    - clear -Hs. simpl in Hs. revert p0 Hs. induction l. discriminate. intros. simpl in Hs. now apply (IHl _ Hs).
+  + destruct (choose s) eqn:H; trivial; [].
+    apply Hchoose_Some in H. rewrite Hs in H. unfold In in H. rewrite empty_spec in H. omega.
 Qed.
 
-Lemma choose_None : forall s, choose s = None <-> s [=] empty.
+
+Lemma fold_nfilter_out_list : forall f x n l s, ~InA eq_key (x, n) l -> NoDupA eq_key l ->
+  multiplicity x (fold_left (fun acc xn => if f (fst xn) (snd xn) : bool
+                                           then add (fst xn) (Pos.to_nat (snd xn)) acc else acc) l s)
+  = multiplicity x s.
 Proof.
-intros s. split; intro Hs.
-+ intro x. unfold choose in Hs. rewrite M.fold_spec in Hs. rewrite empty_spec, multiplicity_out.
-  destruct (M.find x s) eqn:Habs.
-  - rewrite M.find_spec, <- M.bindings_spec1 in Habs. destruct (M.bindings s).
-      now inversion Habs.
-      clear -Hs. simpl in Hs. revert p0 Hs. induction l. discriminate. intros. simpl in Hs. now apply (IHl _ Hs).
-  - reflexivity.
-+ destruct (choose s) eqn:H.
-  - apply choose_Some in H. rewrite Hs in H. unfold In in H. rewrite empty_spec in H. omega.
-  - reflexivity.
+intros f x n l s Hin Hdup. revert s. induction l as [| [y m] l]; intro s; simpl.
++ reflexivity.
++ rewrite IHl.
+  - destruct (f y m); auto. apply m_add_other. intro Habs. apply Hin. now left.
+  - intro Habs. apply Hin. now right.
+  - now inversion_clear Hdup.
+Qed.
+
+Lemma nfilter_spec_In : forall f s s' x, compatb f -> In x s ->
+  multiplicity x
+    (m_fold (fun y n acc => if f y n : bool then add y n acc else acc) s s')
+  = if f x (multiplicity x s) then multiplicity x s + multiplicity x s' else multiplicity x s'.
+Proof.
+intros f s s' x Hf Hin. unfold m_fold. rewrite fold_1. revert s'. unfold In in Hin.
+assert (Hs : InA eq_pair (x, multiplicity x s) (elements s)). { rewrite elements_spec. simpl. now split. }
+assert (Hdup : NoDupA eq_elt (elements s)) by apply elements_NoDupA.
+unfold elements in Hs, Hdup. simpl in Hs, Hdup.
+induction (FMapInterface.elements s); simpl; intro s'; simpl in Hs.
+* exfalso. rewrite <- InA_nil. apply Hs.
+* destruct a as [y m].
+  destruct (equiv_dec (x, Pos.of_nat (multiplicity x s)) (y, m)) as [Heq | Hneq].
+  + destruct Heq as [H1 H2]. simpl in H1, H2 |- *. rewrite H1 in *. subst m.
+    rewrite (fold_nfilter_out_list (fun x y => f x (Pos.to_nat y)) _ (Pos.of_nat (multiplicity y s))).
+    - cbn in Hin. rewrite Nat2Pos.id; try omega; [].
+      destruct (f y (multiplicity y s)) eqn:Htest.
+        now rewrite m_add_same, H1.
+        now rewrite H1.
+    - inversion_clear Hdup. intro Habs. apply H. rewrite InA_map_iff.
+      -- exists (y, Pos.of_nat (multiplicity y s)). split; reflexivity || eassumption.
+      -- autoclass.
+      -- autoclass.
+      -- clear. intros [] [] Hxy. now compute in *.
+    - inversion_clear Hdup. rewrite NoDupA_inj_map in H0; solve [ eassumption | autoclass | now intros [] [] ].
+  + inversion_clear Hs.
+    - elim Hneq. destruct H as [H1 H2]. split; trivial; [].
+      simpl in *. hnf in H2. cbn in H2. now rewrite H2, Pos2Nat.id.
+    - inversion_clear Hdup.
+      assert (Hxy : x =/= y) by (intro; eauto using eq_pair_elt_weak_In).
+      rewrite IHl; try assumption. simpl.
+      destruct (f x (multiplicity x s)), (f y (Pos.to_nat m));
+      reflexivity || rewrite m_add_other; reflexivity || now auto.
+Qed.
+
+Lemma nfilter_spec_out : forall f s s' x, ~In x s ->
+  multiplicity x (m_fold (fun y n acc => if f y n : bool then m_add y n acc else acc) s s')
+  = multiplicity x s'.
+Proof.
+intros f s s' x Hin. unfold m_fold. rewrite fold_1.
+assert (Hs : forall n, ~(InA eq_key_elt (x, n) (FMapInterface.elements s))).
+{ intros n Habs. apply Hin. apply elements_2, find_mapsto_iff in Habs.
+  unfold In. simpl. unfold multiplicity. rewrite Habs. apply Pos2Nat.is_pos. }
+revert s'. induction (FMapInterface.elements s) as [| [y m] l]; intro s'; trivial; [].
+assert ( Hxy : x =/= y). { intro Habs. apply (Hs m). left. now split. }
+simpl. rewrite IHl.
+- destruct (f y (Pos.to_nat m)); trivial; []. apply m_add_other. auto.
+- intros n Habs. apply (Hs n). now right.
+Qed.
+
+Instance filter_spec : FilterSpec elt _.
+Proof.
+assert (Hnfilter : forall (f : elt -> nat -> bool) (x : elt) (s : multiset),
+        Proper (equiv ==> eq ==> eq) f ->
+        (nfilter f s)[x] = (if f x s[x] then s[x] else 0)).
+* intros f x s Hf. unfold nfilter. simpl.
+  destruct (multiplicity x s) eqn:Hin.
+  + rewrite nfilter_spec_out.
+    - unfold multiplicity. rewrite empty_o. now destruct (f x 0).
+    - unfold In. simpl. omega.
+  + rewrite nfilter_spec_In.
+    - unfold multiplicity at 3 4. now rewrite empty_o, Hin, plus_0_r.
+    - assumption.
+    - unfold In. simpl. omega.
+* split; trivial.
+  intros f x s Hf. change (filter f s) with (nfilter (fun x _ => f x) s).
+  apply Hnfilter. repeat intro. now apply Hf.
+Qed.
+
+
+(* Theorem filter_nfilter : forall f s, filter f s [=] nfilter (fun x _ => f x) s.
+Proof. now unfold filter. Qed. *)
+
+Instance sizes_spec : SizeSpec elt _.
+Proof. split.
+* intro. unfold cardinal. simpl. unfold m_fold. reflexivity.
+* intro. unfold size, support. simpl. now rewrite fold_1, fold_left_length, fold_1, fold_left_cons_length.
 Qed.
 
 Lemma fold_and_true_base_step : forall A f (l : list A) b, 
@@ -713,63 +673,73 @@ simpl. intros A f l a b Hl. apply fold_and_true_base_step in Hl.
 destruct (f a). reflexivity. destruct b; simpl in Hl; discriminate Hl.
 Qed.
 
-Lemma for_all_spec_aux : forall (f : M.key -> nat -> bool) s b, compatb f ->
-  (M.fold (fun x n b => b && (f x (Pos.to_nat n))) s b = true
+Lemma Melements_multiplicity : forall s x n,
+  InA eq_key_elt (x, n) (FMapInterface.elements s)
+  <-> multiplicity x s = Pos.to_nat n /\ Pos.to_nat n > 0.
+Proof.
+intros s x n. split; intro H.
++ apply elements_2, find_mapsto_iff in H. unfold multiplicity.
+  rewrite H. split; trivial; []. apply Pos2Nat.is_pos.
++ destruct H as [H1 H2]. unfold multiplicity in H1. destruct (find x s) eqn:Hin.
+  - apply elements_1, find_mapsto_iff. rewrite Hin. f_equal. now apply Pos2Nat.inj.
+  - rewrite  <- H1 in H2. inversion H2.
+Qed.
+
+Lemma for_all_spec_aux : forall (f : elt -> nat -> bool) s b, compatb f ->
+  (m_fold (fun x n b => b && (f x n)) s b = true
    <-> b = true /\ For_all (fun x n => f x n = true) s).
 Proof.
-intros f s b Hf. rewrite M.fold_spec. unfold For_all. split; intro H.
+intros f s b Hf. unfold m_fold. rewrite fold_1. unfold For_all. split; intro H.
 + split. now apply fold_and_true_base_step in H.
-  intros x Hin. rewrite In_MIn in Hin. destruct Hin as [n Hin]. apply M.bindings_spec1 in Hin.
+  intros x Hin. unfold In in Hin. rewrite <- In_MIn in Hin. destruct Hin as [n Hin]. apply elements_1 in Hin.
   assert (Hn : multiplicity x s = Pos.to_nat n) by now rewrite Melements_multiplicity in Hin.
-  revert b H x n Hn Hin. induction (M.bindings s); intros b H x n Hn Hin; inversion_clear Hin.
+  revert b H x n Hn Hin. induction (FMapInterface.elements s); intros b H x n Hn Hin; inversion_clear Hin.
   - simpl in H. apply fold_and_true_base_step in H. rewrite andb_true_iff in H.
     destruct H as [_ H ], a, H0 as [H1 H2]. simpl in *. rewrite Hn, H1. now subst p.
   - simpl in H. apply (IHl _ H _ _ Hn H0).
 + destruct H as [Hb H]. subst b.
-  assert (forall xn, InA (@M.eq_key_elt _) xn (M.bindings s) -> f (fst xn) (Pos.to_nat (snd xn)) = true).
+  assert (forall xn, InA eq_key_elt xn (FMapInterface.elements s) -> f (fst xn) (Pos.to_nat (snd xn)) = true).
   { intros [x n] Hx. simpl. rewrite Melements_multiplicity in Hx. destruct Hx as [Hm Hp].
-    setoid_rewrite <- Pos2Nat.id. rewrite <- Hm. rewrite Nat2Pos.id. apply H. unfold In. now rewrite Hm. omega. }
-  clear H. revert H0. induction (M.bindings s); simpl; intro Hin; trivial.
+    setoid_rewrite <- Pos2Nat.id. rewrite <- Hm, Nat2Pos.id. apply H. unfold In. simpl. now rewrite Hm. omega. }
+  clear H. revert H0. induction (FMapInterface.elements s); simpl; intro Hin; trivial.
   rewrite Hin. apply IHl. intros x Hx. apply Hin. now right. now left.
 Qed.
 
-Corollary for_all_spec : forall f s, compatb f ->
-  (for_all f s = true <-> For_all (fun x n => f x n = true) s).
-Proof. intros. unfold for_all. rewrite for_all_spec_aux; intuition. Qed.
-
-Lemma exists_spec_aux : forall (f : M.key -> nat -> bool) s b, compatb f ->
-  (M.fold (fun x n b => b || (f x (Pos.to_nat n))) s b = true
-   <-> b = true \/ Exists (fun x n => f x n = true) s).
+Lemma exists_spec_aux : forall (f : elt -> nat -> bool) s b, compatb f ->
+  (m_fold (fun x n b => b || (f x n)) s b = true
+  <-> b = true \/ Exists (fun x n => f x n = true) s).
 Proof.
 intros f s b Hf.
 assert (Hequiv : Exists (fun x n => f x n = true) s <->
-        exists x, exists n, InA (@M.eq_key_elt _) (x, n) (M.bindings s) /\ f x (Pos.to_nat n) = true).
+        exists x, exists n, InA eq_key_elt (x, n) (FMapInterface.elements s) /\ f x (Pos.to_nat n) = true).
 { split; intros [x Hx].
-  destruct Hx as [Hin Hfx]. exists x. exists (Pos.of_nat (multiplicity x s)). split.
-    rewrite Melements_multiplicity. unfold In in Hin. simpl. rewrite Nat2Pos.id. now split. omega.
-    rewrite Nat2Pos.id. assumption. unfold In in Hin. omega.
-  destruct Hx as [n [Hin Hfx]]. exists x. rewrite Melements_multiplicity in Hin. destruct Hin as [Hn Hp]. split.
-    simpl in *. unfold In. now rewrite Hn.
-    simpl in *. now rewrite Hn. }
-rewrite Hequiv. clear Hequiv. rewrite M.fold_spec. unfold For_all. split; intro H.
-+ revert b H. induction (M.bindings s); intros b H.
-  - simpl in H. now left.
-  - simpl in H. apply IHl in H. rewrite orb_true_iff in H. destruct H as [[H | H] | H]; (now left) || right.
-      destruct a as [x n]. exists x. exists n. split. now left. assumption.
-      destruct H as [x [n [Hin Hfx]]]. exists x. exists n. split. now right. assumption.  
-+ revert b H. induction (M.bindings s); simpl; intros b H.
-  - destruct H. assumption.
+  + destruct Hx as [Hin Hfx]. exists x. exists (Pos.of_nat (multiplicity x s)). split.
+    - rewrite Melements_multiplicity. unfold In in Hin. simpl in *. rewrite Nat2Pos.id. now split. omega.
+    - rewrite Nat2Pos.id. assumption. unfold In in Hin. simpl in Hin. omega.
+  + destruct Hx as [n [Hin Hfx]]. exists x. rewrite Melements_multiplicity in Hin. destruct Hin as [Hn Hp]. split.
+    - simpl in *. unfold In. simpl. now rewrite Hn.
+    - simpl in *. now rewrite Hn. }
+rewrite Hequiv. clear Hequiv. unfold m_fold. rewrite fold_1. unfold For_all. split; intro H.
+* revert b H. induction (FMapInterface.elements s); intros b H.
+  + simpl in H. now left.
+  + simpl in H. apply IHl in H. rewrite orb_true_iff in H. destruct H as [[H | H] | H]; (now left) || right.
+    - destruct a as [x n]. exists x. exists n. split. now left. assumption.
+    - destruct H as [x [n [Hin Hfx]]]. exists x. exists n. split. now right. assumption.
+* revert b H. induction (FMapInterface.elements s); simpl; intros b H.
+  + destruct H. assumption.
     destruct H as [? [? [Habs _]]]. now inversion Habs.
-  - apply IHl. rewrite orb_true_iff. destruct H as [H | H].
-      now do 2 left.
-      destruct H as [x [n [Hin Hfx]]]. inversion_clear Hin.
-        left. right. destruct H as [H1 H2]. simpl in H1, H2. now rewrite <- H1, <- H2.
-        right. exists x. exists n. now split.
+  + apply IHl. rewrite orb_true_iff. destruct H as [H | H].
+    - now do 2 left.
+    - destruct H as [x [n [Hin Hfx]]]. inversion_clear Hin.
+      -- left. right. destruct H as [H1 H2]. simpl in H1, H2. now rewrite <- H1, <- H2.
+      -- right. exists x. exists n. now split.
 Qed.
 
-Corollary exists_spec : forall f s, compatb f ->
-  (exists_ f s = true <-> Exists (fun x n => f x n = true) s).
-Proof. intros. unfold exists_. rewrite exists_spec_aux; intuition discriminate. Qed.
+Instance quantifiers_spec : QuantifierSpec elt _.
+Proof. split.
+* intros. unfold for_all. simpl. rewrite for_all_spec_aux; intuition.
+* intros. unfold exists_. simpl. rewrite exists_spec_aux; intuition discriminate.
+Qed.
 
 
 Definition npartition_fun f := fun x n acc =>
@@ -778,7 +748,7 @@ Definition npartition_fun f := fun x n acc =>
          else (fst acc, add x (Pos.to_nat n) (snd acc)).
 
 Lemma fold_npartition_fst_out_list : forall f x n l s12,
-  ~InA (@M.eq_key positive) (x, n) l -> NoDupA (@M.eq_key _) l ->
+  ~InA eq_key (x, n) l -> NoDupA eq_key l ->
   multiplicity x
   (fst
      (fold_left (fun acc xn => if f (fst xn) (Pos.to_nat (snd xn)) : bool
@@ -786,88 +756,69 @@ Lemma fold_npartition_fst_out_list : forall f x n l s12,
          else (fst acc, add (fst xn) (Pos.to_nat (snd xn)) (snd acc))) l s12))
   = multiplicity x (fst s12).
 Proof.
-intros f x n l s12 Hin Hdup. revert s12. induction l as [| [y m] l]; intros s12; simpl.
-  reflexivity.
-  rewrite IHl.
-    destruct (f y (Pos.to_nat m)); simpl.
-      apply add_other. intro Habs. apply Hin. left. compute. auto. auto.
-    intro Habs. apply Hin. now right.
-    now inversion_clear Hdup.
+intros f x n l s12 Hin Hdup. revert s12. induction l as [| [y m] l]; intros s12; trivial.
+simpl. rewrite IHl.
+- destruct (f y (Pos.to_nat m)); trivial; [].
+  apply m_add_other. intro Habs. apply Hin. now left.
+- intro Habs. apply Hin. now right.
+- now inversion_clear Hdup.
 Qed.
 
-Lemma npartition_spec_fst_In : forall f (s : t) (s12 : t * t) x, compatb f -> In x s ->
-  multiplicity x (fst (M.fold (fun x n acc =>
-         if f x (Pos.to_nat n) : bool
-         then (add x (Pos.to_nat n) (fst acc), snd acc)
-         else (fst acc, add x (Pos.to_nat n) (snd acc))) s s12)) =
+Lemma npartition_spec_fst_In : forall f s s12 x, compatb f -> In x s ->
+  multiplicity x (fst (m_fold (fun x n acc =>
+         if f x n : bool
+         then (m_add x n (fst acc), snd acc)
+         else (fst acc, m_add x n (snd acc))) s s12)) =
   (if f x (multiplicity x s) then multiplicity x s + multiplicity x (fst s12) else multiplicity x (fst s12)).
 Proof.
-intros f s s' x Hf Hin. rewrite M.fold_spec. revert s'. unfold In in Hin.
-assert (Hs : InA (@M.eq_key_elt _) (x, multiplicity x s) (elements s)). { rewrite elements_spec. simpl. now split. }
-assert (Hdup : NoDupA (@M.eq_key _) (elements s)) by apply elements_NoDupA.
-unfold elements in Hs, Hdup.
-induction (M.bindings s); simpl; intros [s1 s2]; simpl in Hs.
+intros f s s' x Hf Hin. unfold m_fold. rewrite fold_1. revert s'. unfold In in Hin. simpl in Hin.
+assert (Hs : InA eq_pair (x, multiplicity x s) (elements s)). { rewrite elements_spec. simpl. now split. }
+assert (Hdup : NoDupA eq_elt (elements s)) by apply elements_NoDupA.
+unfold elements in Hs, Hdup. simpl in Hs, Hdup.
+induction (FMapInterface.elements s); simpl; intros [s1 s2]; simpl in Hs.
 * exfalso. rewrite <- InA_nil. apply Hs.
 * destruct a as [y m].
-  destruct (Meq_dec (x, Pos.of_nat (multiplicity x s)) (y, m)) as [Heq | Hneq].
+  destruct (equiv_dec (x, Pos.of_nat (multiplicity x s)) (y, m)) as [Heq | Hneq].
   + destruct Heq as [H1 H2]. simpl in H1, H2 |- *. rewrite H1 in *. subst m.
     rewrite (fold_npartition_fst_out_list f _ (Pos.of_nat (multiplicity y s))).
-    - unfold npartition_fun. rewrite Nat2Pos.id; try omega.
-      destruct (f y (multiplicity y s)) eqn:Htest; simpl.
-        rewrite add_same, H1. now apply plus_comm.
-        now rewrite H1.
+    - unfold npartition_fun. rewrite Nat2Pos.id; try omega; [].
+      destruct (f y (multiplicity y s)) eqn:Htest; simpl; now rewrite ?m_add_same, H1.
     - inversion_clear Hdup. intro Habs. apply H. rewrite InA_map_iff.
-        exists (y, Pos.of_nat (multiplicity y s)). split. reflexivity. eassumption.
-        apply Meq_key_equiv.
-        apply Meq_key_equiv.
-        clear. intros [] [] Hxy. now compute in *.
-    - inversion_clear Hdup. rewrite NoDupA_inj_map in H0.
-        eassumption.
-        now apply Meq_key_equiv.
-        now apply Meq_key_equiv.
-        now intros [] [].
-        now intros [] [].
+      -- exists (y, Pos.of_nat (multiplicity y s)). split; eauto; reflexivity.
+      -- autoclass.
+      -- autoclass.
+      -- clear. intros [] [] Hxy. now compute in *.
+    - inversion_clear Hdup. rewrite NoDupA_inj_map in H0;
+       solve [ eassumption | autoclass | now intros [] [] ].
   + inversion_clear Hs.
-    - elim Hneq. destruct H. split. assumption. simpl in *. now rewrite H0, Pos2Nat.id.
-    - inversion_clear Hdup. assert (Hxy : ~E.eq x y).
-      { intro Habs. apply H0. now apply (eq_key_elt_eq_key_weak_In _ x y (multiplicity x s)). }
+    - elim Hneq. destruct H as [H1 H2]. split. assumption. hnf in *. simpl in *. now rewrite H2, Pos2Nat.id.
+    - inversion_clear Hdup.
+      assert (Hxy : x =/= y) by (intro; eauto using eq_pair_elt_weak_In).
       rewrite IHl; try assumption. simpl. unfold npartition_fun.
       destruct (f x (multiplicity x s)), (f y (Pos.to_nat m));
-      reflexivity || simpl; rewrite add_other; reflexivity || now auto.
+      reflexivity || simpl; rewrite m_add_other; reflexivity || now auto.
 Qed.
 
 Lemma npartition_spec_fst_out : forall f s s12 x, ~In x s ->
-  multiplicity x (fst (M.fold (fun x n acc =>
-         if f x (Pos.to_nat n) : bool
-         then (add x (Pos.to_nat n) (fst acc), snd acc)
-         else (fst acc, add x (Pos.to_nat n) (snd acc))) s s12)) = multiplicity x (fst s12).
+  multiplicity x (fst (m_fold (fun x n acc =>
+      if f x n : bool then (m_add x n (fst acc), snd acc) else (fst acc, m_add x n (snd acc))) s s12))
+  = multiplicity x (fst s12).
 Proof.
-intros f s s' x Hin. rewrite M.fold_spec.
-assert (Hs : forall n, ~(InA (@M.eq_key_elt _) (x, n) (M.bindings s))).
-{ intros n Habs. apply Hin. rewrite M.bindings_spec1, <- M.find_spec in Habs.
-  unfold In, multiplicity. rewrite Habs. apply Pos2Nat.is_pos. }
-revert s'. induction (M.bindings s) as [| [y m] l]; intro s'; simpl.
-  reflexivity.
-  assert ( Hxy : ~E.eq x y). { intro Habs. apply (Hs m). left. now split. }
-  rewrite IHl. unfold npartition_fun. destruct (f y (Pos.to_nat m)). apply add_other. now auto. reflexivity.
-  intros n Habs. apply (Hs n). now right.
-Qed.
-
-Corollary npartition_spec_fst : forall f s, compatb f -> fst (npartition f s) [=] nfilter f s.
-Proof.
-intros f s Hf x. unfold npartition. rewrite nfilter_spec; trivial.
-destruct (multiplicity x s) eqn:Hin.
-  rewrite npartition_spec_fst_out.
-    now destruct (f x 0); apply empty_spec.
-    unfold In. omega.
-  rewrite npartition_spec_fst_In.
-    now rewrite empty_spec, Hin, plus_0_r.
-    assumption.
-    unfold In. rewrite Hin. omega.
+intros f s s' x Hin. unfold m_fold. rewrite fold_1.
+assert (Hs : forall n, ~(InA eq_key_elt (x, n) (FMapInterface.elements s))).
+{ intros n Habs. apply Hin. apply elements_2, find_mapsto_iff in Habs.
+  unfold In. simpl. unfold multiplicity. rewrite Habs. apply Pos2Nat.is_pos. }
+revert s'. induction (FMapInterface.elements s) as [| [y m] l]; intro s'; simpl; trivial; [].
+assert ( Hxy : x =/= y). { intro Habs. apply (Hs m). left. now split. }
+rewrite IHl.
++ unfold npartition_fun. destruct (f y (Pos.to_nat m)).
+  - apply m_add_other. now auto.
+  - reflexivity.
++ intros n Habs. apply (Hs n). now right.
 Qed.
 
 Lemma fold_npartition_snd_out_list : forall f x n l s12,
-  ~InA (@M.eq_key positive) (x, n) l -> NoDupA (@M.eq_key _) l ->
+  ~InA eq_key (x, n) l -> NoDupA eq_key l ->
   multiplicity x
   (snd
      (fold_left
@@ -877,132 +828,112 @@ Lemma fold_npartition_snd_out_list : forall f x n l s12,
          else (fst acc, add (fst xn) (Pos.to_nat (snd xn)) (snd acc))) l s12))
   = multiplicity x (snd s12).
 Proof.
-intros f x n l s12 Hin Hdup. revert s12. induction l as [| [y m] l]; intros s12; simpl.
-  reflexivity.
-  rewrite IHl.
-    destruct (f y (Pos.to_nat m)). reflexivity. simpl. apply add_other. intro Habs. apply Hin. left. compute. auto.
-    intro Habs. apply Hin. now right.
-    now inversion_clear Hdup.
+intros f x n l s12 Hin Hdup. revert s12.
+induction l as [| [y m] l]; intros s12; simpl.
++ reflexivity.
++ rewrite IHl.
+  - destruct (f y (Pos.to_nat m)). reflexivity. simpl. apply m_add_other. intro Habs. apply Hin. now left.
+  - intro Habs. apply Hin. now right.
+  - now inversion_clear Hdup.
 Qed.
 
-Lemma npartition_spec_snd_In : forall f (s : t) (s12 : t * t) x, compatb f -> In x s ->
+Lemma npartition_spec_snd_In : forall f s s12 x, compatb f -> In x s ->
   multiplicity x
   (snd
-     (M.fold
+     (m_fold
         (fun y n acc =>
-         if f y (Pos.to_nat n) : bool
-         then (add y (Pos.to_nat n) (fst acc), snd acc)
-         else (fst acc, add y (Pos.to_nat n) (snd acc))) s s12)) =
-  (if f x (multiplicity x s) then multiplicity x (snd s12) else multiplicity x s + multiplicity x (snd s12)).
+         if f y n : bool then (m_add y n (fst acc), snd acc) else (fst acc, m_add y n (snd acc))) s s12))
+  = if f x (multiplicity x s) then multiplicity x (snd s12) else multiplicity x s + multiplicity x (snd s12).
 Proof.
-intros f s s' x Hf Hin. rewrite M.fold_spec. revert s'. unfold In in Hin.
-assert (Hs : InA (@M.eq_key_elt _) (x, multiplicity x s) (elements s)). { rewrite elements_spec. simpl. now split. }
-assert (Hdup : NoDupA (@M.eq_key _) (elements s)) by apply elements_NoDupA.
-unfold elements in Hs, Hdup.
-induction (M.bindings s); simpl; intros [s1 s2]; simpl in Hs.
+intros f s s' x Hf Hin. unfold m_fold. rewrite fold_1. revert s'. unfold In in Hin. simpl in Hin.
+assert (Hs : InA eq_pair (x, multiplicity x s) (elements s)). { rewrite elements_spec. simpl. now split. }
+assert (Hdup : NoDupA eq_elt (elements s)) by apply elements_NoDupA.
+unfold elements in Hs, Hdup. simpl in Hs, Hdup.
+induction (FMapInterface.elements s); simpl; intros [s1 s2]; simpl in Hs.
 * exfalso. rewrite <- InA_nil. apply Hs.
 * destruct a as [y m].
-  destruct (Meq_dec (x, Pos.of_nat (multiplicity x s)) (y, m)) as [Heq | Hneq].
+  destruct (equiv_dec (x, Pos.of_nat (multiplicity x s)) (y, m)) as [Heq | Hneq].
   + destruct Heq as [H1 H2]. simpl in H1, H2 |- *. rewrite H1 in *. subst m.
     rewrite (fold_npartition_snd_out_list f _ (Pos.of_nat (multiplicity y s))).
-    - rewrite Nat2Pos.id; try omega.
-      destruct (f y (multiplicity y s)) eqn:Htest; simpl.
-        now rewrite H1.
-        rewrite add_same, H1. now apply plus_comm.
+    - rewrite Nat2Pos.id; try omega; [].
+      destruct (f y (multiplicity y s)) eqn:Htest; simpl; now rewrite ?m_add_same, H1.
     - inversion_clear Hdup. intro Habs. apply H. rewrite InA_map_iff.
-        exists (y, Pos.of_nat (multiplicity y s)). split. reflexivity. eassumption.
-        apply Meq_key_equiv.
-        apply Meq_key_equiv.
-        clear. intros [] [] Hxy. now compute in *.
-    - inversion_clear Hdup. rewrite NoDupA_inj_map in H0.
-        eassumption.
-        now apply Meq_key_equiv.
-        now apply Meq_key_equiv.
-        now intros [] [].
-        now intros [] [].
+      -- exists (y, Pos.of_nat (multiplicity y s)). split; reflexivity || eassumption.
+      -- autoclass.
+      -- autoclass.
+      -- clear. intros [] [] Hxy. now compute in *.
+    - inversion_clear Hdup. rewrite NoDupA_inj_map in H0;
+      solve [eassumption | autoclass | now intros [] [] ].
   + inversion_clear Hs.
-    - elim Hneq. destruct H. split. assumption. simpl in *. now rewrite H0, Pos2Nat.id.
-    - inversion_clear Hdup. assert (Hxy : ~E.eq x y).
-      { intro Habs. apply H0. now apply (eq_key_elt_eq_key_weak_In _ x y (multiplicity x s)). }
+    - elim Hneq. destruct H as [H1 H2]. split. assumption. hnf in *. simpl in *. now rewrite H2, Pos2Nat.id.
+    - inversion_clear Hdup.
+      assert (Hxy : x =/= y) by (intro; eauto using eq_pair_elt_weak_In).
       rewrite IHl; try assumption. simpl.
       destruct (f x (multiplicity x s)), (f y (Pos.to_nat m));
-      reflexivity || simpl; rewrite add_other; reflexivity || now auto.
+      reflexivity || simpl; rewrite m_add_other; reflexivity || now auto.
 Qed.
 
 Lemma npartition_spec_snd_out : forall f s s12 x, ~In x s ->
   multiplicity x
   (snd
-     (M.fold
+     (m_fold
         (fun y n acc =>
-         if f y (Pos.to_nat n) : bool
-         then (add y (Pos.to_nat n) (fst acc), snd acc)
-         else (fst acc, add y (Pos.to_nat n) (snd acc))) s s12)) =
-  multiplicity x (snd s12).
+         if f y n : bool then (m_add y n (fst acc), snd acc) else (fst acc, m_add y n (snd acc))) s s12))
+  = multiplicity x (snd s12).
 Proof.
-intros f s s' x Hin. rewrite M.fold_spec.
-assert (Hs : forall n, ~(InA (@M.eq_key_elt _) (x, n) (M.bindings s))).
-{ intros n Habs. apply Hin. rewrite M.bindings_spec1, <- M.find_spec in Habs.
-  unfold In, multiplicity. rewrite Habs. apply Pos2Nat.is_pos. }
-revert s'. induction (M.bindings s) as [| [y m] l]; intro s'; simpl.
-  reflexivity.
-  assert ( Hxy : ~E.eq x y). { intro Habs. apply (Hs m). left. now split. }
-  rewrite IHl. destruct (f y (Pos.to_nat m)); simpl. reflexivity. apply add_other. now auto.
-  intros n Habs. apply (Hs n). now right.
+intros f s s' x Hin. unfold m_fold. rewrite fold_1.
+assert (Hs : forall n, ~(InA eq_key_elt (x, n) (FMapInterface.elements s))).
+{ intros n Habs. apply Hin. apply elements_2, find_mapsto_iff in Habs.
+  unfold In. simpl. unfold multiplicity. rewrite Habs. apply Pos2Nat.is_pos. }
+revert s'. induction (FMapInterface.elements s) as [| [y m] l]; intro s'; trivial.
+assert (Hxy : x =/= y). { intro Habs. apply (Hs m). left. now split. }
+simpl. rewrite IHl.
+- destruct (f y (Pos.to_nat m)); trivial; [].
+  apply m_add_other. now auto.
+- intros n Habs. apply (Hs n). now right.
 Qed.
 
-Corollary npartition_spec_snd : forall f s,
-  compatb f -> snd (npartition f s) [=] nfilter (fun x n => negb (f x n)) s.
-Proof.
-intros f s Hf x. unfold npartition. rewrite nfilter_spec.
-destruct (multiplicity x s) eqn:Hin.
-  rewrite npartition_spec_snd_out.
-    now destruct (f x 0); apply empty_spec.
-    unfold In. omega.
-  rewrite npartition_spec_snd_In.
-    rewrite empty_spec, Hin, plus_0_r. now destruct (f x (S n)).
-    assumption.
-    unfold In. rewrite Hin. omega.
-    intros ? ? Heq ? ? ?. subst. now rewrite Heq.
+Instance npartition_spec : NpartitionSpec elt _.
+Proof. split.
+* intros f s Hf x. unfold npartition. rewrite nfilter_spec; trivial. simpl.
+  destruct (multiplicity x s) eqn:Hin.
+  + rewrite npartition_spec_fst_out.
+    - simpl. unfold multiplicity. rewrite empty_o. now destruct (f x 0).
+    - unfold In. simpl. omega.
+  + rewrite npartition_spec_fst_In.
+    - simpl. unfold multiplicity at 3 4. now rewrite empty_o, Hin, plus_0_r.
+    - assumption.
+    - unfold In. simpl. omega.
+* intros f s Hf x. rewrite nfilter_spec.
+  + unfold npartition. simpl.
+    destruct (multiplicity x s) eqn:Hin.
+    - rewrite npartition_spec_snd_out.
+      -- simpl. unfold multiplicity. rewrite empty_o. now destruct (f x 0).
+      -- unfold In. simpl. omega.
+    - rewrite npartition_spec_snd_In.
+      -- simpl. unfold multiplicity at 2 4. rewrite empty_o, Hin, plus_0_r. now destruct (f x (S n)).
+      -- assumption.
+      -- unfold In. simpl. omega.
+  + intros ? ? Heq ? ? ?. subst. now rewrite Heq.
 Qed.
 
-Theorem partition_npartition_fst : forall f s, fst (partition f s) [=] fst (npartition (fun x _ => f x) s).
+Theorem partition_npartition_fst : forall f s, fst (partition f s) == fst (npartition (fun x _ => f x) s).
 Proof. now unfold partition. Qed.
 
-Theorem partition_npartition_snd : forall f s, snd (partition f s) [=] snd (npartition (fun x _ => f x) s).
+Theorem partition_npartition_snd : forall f s, snd (partition f s) == snd (npartition (fun x _ => f x) s).
 Proof. now unfold partition. Qed.
 
-Corollary partition_spec_fst : forall f s, Proper (E.eq ==> Logic.eq) f -> fst (partition f s) [=] filter f s.
-Proof.
-intros f s Hf. rewrite partition_npartition_fst, npartition_spec_fst.
-- reflexivity.
-- repeat intro. now apply Hf.
+Instance partition_spec : PartitionSpec elt _.
+Proof. split.
+* intros f s Hf. rewrite partition_npartition_fst, npartition_spec_fst.
+  - reflexivity.
+  - repeat intro. now apply Hf.
+* intros f s Hf. rewrite partition_npartition_snd, npartition_spec_snd.
+  - reflexivity.
+  - repeat intro. now apply Hf.
 Qed.
 
-Corollary partition_spec_snd : forall f s, Proper (E.eq ==> Logic.eq) f ->
-  snd (partition f s) [=] filter (fun x => negb (f x)) s.
-Proof.
-intros f s Hf. rewrite partition_npartition_snd, npartition_spec_snd.
-- reflexivity.
-- repeat intro. now apply Hf.
-Qed.
+Instance FMultisetsFacts : FMultisetsOn elt FMOps_WMap.
+Proof. split; autoclass. Qed.
 
-Instance fold_compat A (eqA : A -> A -> Prop) `{Equivalence A eqA} : forall f,
-  Proper (E.eq ==> Logic.eq ==> eqA ==> eqA) f -> transpose2 eqA f ->
-  Proper (eq ==> eqA ==> eqA) (fold f).
-Proof.
-intros f Hf Hfcomm s1 s2 Hs x y Hxy. unfold fold. do 2 rewrite M.fold_spec.
-rewrite fold_left_symmetry_PermutationA.
-+ reflexivity.
-+ now apply Meq_equiv.
-+ assumption.
-+ repeat intro. now apply Hf; rewrite H1 || rewrite H0.
-+ intros. apply Hfcomm.
-+ apply NoDupA_equivlistA_PermutationA.
-  - now apply Meq_equiv.
-  - eapply NoDupA_strengthen; try apply M.bindings_spec2w. now intros [? ?] [? ?] [? ?].
-  - eapply NoDupA_strengthen; try apply M.bindings_spec2w. now intros [? ?] [? ?] [? ?].
-  - clear -Hs. intros [x n]. do 2 rewrite Melements_multiplicity. now rewrite Hs.
-+ assumption.
-Qed.
-
-End FMultisets.
+End WMapImplementation.
